142. $\cfrac{\sqrt{x}+1}{2\sqrt{x}-1}=\cfrac{x+3\sqrt{x}+2}{\sqrt{x}}\Leftrightarrow
\begin{cases}\cfrac{t+1}{2t-1}=\cfrac{t^2+3t+2}{t},\\ t=\sqrt{x}\geqslant0.\end{cases}\Leftrightarrow
\begin{cases}\cfrac{t+1}{2t-1}=\cfrac{(t+1)(t+2)}{t},\\ t=\sqrt{x}\geqslant0.\end{cases}\Leftrightarrow$\\$
\begin{cases}\cfrac{1}{2t-1}=\cfrac{t+2}{t},\\ t=\sqrt{x}\geqslant0.\end{cases}\Leftrightarrow
\begin{cases}t=2t^2+4t-t-2,\\ t=\sqrt{x}>0,\ t
eq\cfrac{1}{2}.\end{cases}\Leftrightarrow
\begin{cases}t^2+t-1=0,\\ t=\sqrt{x}>0,\ t
eq\cfrac{1}{2}.\end{cases}\Leftrightarrow
\begin{cases}t=\cfrac{-1\pm\sqrt{5}}{2},\\ t=\sqrt{x}>0,\ t
eq\cfrac{1}{2}.\end{cases}
\Leftrightarrow x=\left(\cfrac{-1+\sqrt{5}}{2}
ight)^2=
\cfrac{1-2\sqrt{5}+5}{4}=\cfrac{3-\sqrt{5}}{2}.$\\
