124. $(x^2+x-2)\sqrt{x+1}=(x-1)(x^2+3x+2)\Leftrightarrow(x-1)(x+2)\sqrt{x+1}=(x-1)(x+2)(x+1)\Leftrightarrow
(x-1)(x+2)(\sqrt{x+1}-x-1)=0\Leftrightarrow
\begin{cases}\left[\begin{array}{l} x=1,\\ x=-2,\\ \sqrt{x+1}=x+1.\end{array}
ight.\\ x\geqslant-1.\end{cases}\Leftrightarrow
\begin{cases}\left[\begin{array}{l} x=1,\\ x+1=x^2+2x+1.\end{array}
ight.\\ x\geqslant-1.\end{cases}\Leftrightarrow
\begin{cases}\left[\begin{array}{l} x=1,\\ x(x+1)=0.\end{array}
ight.\\ x\geqslant-1.\end{cases}\Leftrightarrow x\in\{-1;0;1\}$\\
