75. $\cfrac{x^2+4}{x}+\cfrac{x}{x^2+3x+4}+\cfrac{11}{2}=0\Leftrightarrow x+\cfrac{4}{x}+\cfrac{1}{x+\cfrac{4}{x}+3}+\cfrac{11}{2}=0.$ Сделаем замену $t=x+\cfrac{4}{x},$ тогда $t+\cfrac{1}{t+3}+\cfrac{11}{2}=0,\ t^2+3t+1+\cfrac{11}{2}t+\cfrac{33}{2}=0,\ t^2+\cfrac{17}{2}t+\cfrac{35}{2}=0,\
2t^2+17t+35=0,\ (2t+7)(t+5)=0,\ t=-5$ или $t=-\cfrac{7}{2}.$ В первом случае $x+\cfrac{4}{x}=-5,\ x^2+4=-5x,\ x^2+5x+4=0,\ (x+4)(x+1)=0,\ x=-4$ или $x=-1.$ Во втором случае $x+\cfrac{4}{x}=-\cfrac{7}{2},\ x^2+4=-\cfrac{7}{2}x,\ x^2+\cfrac{7}{2}x+4=0,\ x\in\{\varnothing\}.$\\
