131. $2\cdot(x^2+2x-5)^2+3x^2+6x=69\Leftrightarrow2\cdot(x^2+2x-5)^2+3\cdot(x^2+2x-5)=54\Leftrightarrow\begin{cases}x^2+2x-5=t,\\ 2t^2+3t-54=0.\end{cases}\Leftrightarrow
\begin{cases}x^2+2x-5=t,\\ (2t-9)(t+6)=0.\end{cases}\Leftrightarrow\left[\begin{array}{l}x^2+2x-5=\cfrac{9}{2},\\x^2+2x-5=-6.\end{array}
ight.
\Leftrightarrow\left[\begin{array}{l}2x^2+4x-19=0,\\x^2+2x+1=0.\end{array}
ight.\Leftrightarrow \left[\begin{array}{l}2x^2+4x-19=0,\\(x+1)^2=0.\end{array}
ight.\Leftrightarrow
x\in\left\{\cfrac{-2\pm\sqrt{42}}{2};-1
ight\}.$\\
