37. $\cfrac{\left(-1\cfrac{4}{5}-6\cfrac{1}{3}+8,75\right):1\cfrac{2}{3}-\cfrac{-2,08}{16}}
{-1\cfrac{7}{25}:1,92+\cfrac{7}{22}\cdot\left(-3\cfrac{2}{3}\right)}=
\cfrac{\left(1-\cfrac{4}{5}-\cfrac{1}{3}+\cfrac{3}{4}\right):\cfrac{5}{3}+\cfrac{208}{1600}}
{-\cfrac{32}{25}:\cfrac{192}{100}-\cfrac{7}{22}\cdot\cfrac{11}{3}}=
\cfrac{\cfrac{37}{60}\cdot\cfrac{3}{5}+\cfrac{208}{1600}}
{-\cfrac{32}{25}\cdot\cfrac{100}{192}-\cfrac{7}{6}}=$\\$=
\cfrac{\cfrac{37}{100}+\cfrac{13}{100}}
{-\cfrac{2}{3}-\cfrac{7}{6}}=\cfrac{\cfrac{1}{2}}{-\cfrac{11}{6}}=-\cfrac{3}{11}.$\\