17. $\cfrac{5\cdot\left(\cfrac{26}{35}-3,75:8\cfrac{3}{4}\right)}{\left(13:1\cfrac{2}{3}-0,3:\cfrac{1}{18}\right)\cdot3\cfrac{4}{7}}=
\cfrac{5\cdot\left(\cfrac{26}{35}-\cfrac{375}{100}\cdot\cfrac{4}{35}\right)}{\left(13\cdot\cfrac{3}{5}-\cfrac{3}{10}\cdot\cfrac{18}{1}\right)\cdot\cfrac{25}{7}}=
\cfrac{5\cdot\left(\cfrac{26}{35}-\cfrac{3}{7}\right)}{\left(\cfrac{39}{5}-\cfrac{27}{5}\right)\cdot\cfrac{25}{7}}=
\cfrac{5\cdot\cfrac{11}{35}}{\cfrac{12}{5}\cdot\cfrac{25}{7}}=\cfrac{\cfrac{11}{7}}{\cfrac{60}{7}}=\cfrac{11}{60}.$\\
