\section{Преобразование буквенных выражений решения}
1. $\sqrt{4x^2-4x+1}+\sqrt{16x^2-8x+1}=\sqrt{(2x-1)^2}+\sqrt{(4x-1)^2}=|2x-1|+|4x-1|=1-2x+4x-1=2x.$\\
2. $\sqrt{25x^2+10x+1}+\sqrt{9x^2+6x+1}=\sqrt{(5x+1)^2}+\sqrt{(3x+1)^2}=|5x+1|+|3x+1|=-5x-1+3x+1=-2x.$\\
3. $\cfrac{(5a-4)^2+2(5a-4)(4-3a)+(3a-4)^2}{(2a+5)^2-2(2a+5)(5-3a)+(3a-5)^2}=
\cfrac{(5a-4+4-3a)^2}{(2a+5-5+3a)^2}=\cfrac{4a^2}{25a^2}=\cfrac{4}{25}.$\\
4. $\cfrac{(4b-5)^2+2(4b-5)(5-b)+(b-5)^2}{(7b+4)^2-2(7b+4)(4-3b)+(3b-4)^2}=
\cfrac{(4b-5+5-b)^2}{(7b+4-4+3b)^2}=\cfrac{9b^2}{100b^2}=\cfrac{9}{100}.$\\
5. $\cfrac{a-b}{a-3\sqrt{ab}+2b}=[x=\sqrt{a},\ y=\sqrt{b}]=\cfrac{x^2-y^2}{x^2-3xy+2y^2}=\cfrac{(x-y)(x+y)}{x(x-y)-2y(x-y)}=\cfrac{x+y}{x-2y}=\cfrac{\sqrt{a}+\sqrt{b}}{\sqrt{a}-2\sqrt{b}}.$\\
6. $\cfrac{x+4\sqrt{xy}+3y}{x-y}=[a=\sqrt{x},\ b=\sqrt{y}]=\cfrac{a^2+4ab+3b^2}{a^2-b^2}=\cfrac{a(a+b)+3b(a+b)}{(a-b)(a+b)}=\cfrac{a+3b}{a-b}=
\cfrac{\sqrt{x}+3\sqrt{y}}{\sqrt{x}-\sqrt{y}}.$\\
7. $\cfrac{x^4-2x^3+x-2}{x^3-3x^2+3x-2}=\cfrac{x^3(x-2)+x-2}{x^3-3x^2+3x-1-1}=\cfrac{(x^3+1)(x-2)}{(x-1)^3-1}=
\cfrac{(x+1)(x^2-x+1)(x-2)}{(x-2)(x^2-2x+1+x-1+1)}=x+1.$\\
8. $\cfrac{x^6+x^4-x^2-1}{x^3+x^2+x+1}=\cfrac{x^4(x^2+1)-(x^2+1)}{x^2(x+1)+x+1}=\cfrac{(x^2+1)(x^4-1)}{(x^2+1)(x+1)}=\cfrac{(x^2-1)(x^2+1)}{x+1}=$\\$=
\cfrac{(x-1)(x+1)(x^2+1)}{x+1}=(x-1)(x^2+1).$\\
9. $\left(\cfrac{\sqrt{a}+1}{\sqrt{a}-1}-\cfrac{\sqrt{a}-1}{\sqrt{a}+1}+4\sqrt{a}
ight)\cdot
\left(\sqrt{\cfrac{a}{4}}-\sqrt{\cfrac{1}{4a}}
ight)=[x=\sqrt{a}]=
\left(\cfrac{x+1}{x-1}-\cfrac{x-1}{x+1}+4x
ight)\cdot
\left(\cfrac{x}{2}-\cfrac{1}{2x}
ight)=$\\
$=\cfrac{x^2+2x+1-x^2+2x-1+4x^3-4x}{(x-1)(x+1)}\cdot\cfrac{x^2-1}{2x}=2x^2=2a.$\\
10. $\left(\cfrac{\sqrt{a}}{\sqrt{a}+\sqrt{b}}+\cfrac{\sqrt{b}}{\sqrt{a}-\sqrt{b}}+
\cfrac{2\sqrt{ab}}{a-b}
ight)\cdot\left(\sqrt{a}-\cfrac{\sqrt{ab}+b}{\sqrt{a}+\sqrt{b}}
ight)=[x=\sqrt{a},\ y=\sqrt{b}]=$\\$=
\left(\cfrac{x}{x+y}+\cfrac{y}{x-y}+
\cfrac{2xy}{x^2-y^2}
ight)\cdot\left(x-\cfrac{xy+y^2}{x+y}
ight)=\cfrac{x^2-xy+xy+y^2+2xy}{(x-y)(x+y)}\cdot\left(x-\cfrac{y(x+y)}{x+y}
ight)=$\\$=
\cfrac{x^2-xy+xy+y^2+2xy}{(x-y)(x+y)}\cdot(x-y)=\cfrac{x^2+2xy+y^2}{x+y}=\cfrac{(x+y)^2}{x+y}=x+y=\sqrt{a}+\sqrt{b}.$\\
11. $a^3-7a+6=a(a^2-1)-6(a-1)=a(a-1)(a+1)-6(a-1)=(a-1)(a^2+a-6)=(a-1)(a^2-4+a-2)=(a-1)((a-2)(a+2)+a-2)=(a-1)(a-2)(a+3).$\\
12. $a^3-7a-6=a(a^2-1)-6(a+1)=a(a-1)(a+1)-6(a+1)=(a+1)(a^2-a-6)=(a-1)(a^2-4-(a+2))=(a+1)((a-2)(a+2)-(a+2))=(a+1)(a+2)(a-3).$\\
13. $\cfrac{a^4+4}{(a+1)^2+1}=\cfrac{a^4+4a^2+4-4a^2}{a^2+2a+1+1}=\cfrac{(a^2+2)^2-(2a)^2}{a^2+2a+2}=\cfrac{(a^2-2a+2)(a^2+2a+2)}{a^2+2a+2}=a^2-2a+2.$\\
14. $\cfrac{b^4+64}{(b-2)^2+4}=\cfrac{b^4+16b^2+64-16b^2}{b^2-4b+4+4}=\cfrac{(b^2+8)^2-(4b)^2}{b^2-4b+8}=\cfrac{(b^2-4b+8)(b^2+4b+8)}{b^2-4b+8}=b^2+4b+8.$\\
15. $\left(\sqrt{a}+\cfrac{b}{\sqrt{a}-\sqrt{b}}
ight)\cdot\left(1-\cfrac{\sqrt{b^3}}{a\sqrt{a}+b\sqrt{b}}
ight)\cdot
(\sqrt{a}+\sqrt{b})=[x=\sqrt{a},\ y=\sqrt{b}]=$\\$=\left(x+\cfrac{y^2}{x-y}
ight)\cdot\left(1-\cfrac{y^3}{x^3+y^3}
ight)\cdot(x+y)=
\cfrac{x^2-xy+y^2}{x-y}\cdot\cfrac{x^3+y^3-y^3}{(x+y)(x^2-xy+y^2)}\cdot(x+y)=\cfrac{x^3}{x-y}=\cfrac{a\sqrt{a}}{\sqrt{a}-\sqrt{b}}.$\\
16. $\left(\sqrt{a}+\cfrac{b}{\sqrt{a}+\sqrt{b}}
ight)\cdot\left(1+\cfrac{\sqrt{b^3}}{a\sqrt{a}-b\sqrt{b}}
ight)\cdot
(\sqrt{a}-\sqrt{b})=[x=\sqrt{a},\ y=\sqrt{b}]=$\\$=\left(x+\cfrac{y^2}{x+y}
ight)\cdot\left(1+\cfrac{y^3}{x^3-y^3}
ight)\cdot
(x-y)=\cfrac{x^2+xy+y^2}{x+y}\cdot\cfrac{x^3-y^3+y^3}{(x-y)(x^2+xy+y^2)}\cdot(x-y)=\cfrac{x^3}{x+y}=\cfrac{a\sqrt{a}}{\sqrt{a}-\sqrt{b}}.$\\
17. $\cfrac{a+1}{a^4+a^3+a^2}: \cfrac{1}{a^5-a^2}=\cfrac{a+1}{a^2(a^2+a+1)}\cdot\cfrac{a^2(a-1)(a^2+a+1)}{1}=a^2-1.$\\
18. $\cfrac{a-1}{a^4-a^3+a^2}: \cfrac{1}{a^5+a^2}=\cfrac{a-1}{a^2(a^2-a+1)}\cdot\cfrac{a^2(a+1)(a^2-a+1)}{1}=a^2-1.$\\
19. $a^3+2a-3=a^3-1+2(a-1)=(a-1)(a^2+a+1)+2(a-1)=(a-1)(a^2+a+3).$\\
20. $a^3+3a-4=a^3-1+3(a-1)=(a-1)(a^2+a+1)+3(a-1)=(a-1)(a^2+a+4).$\\
21. $\cfrac{m\sqrt{m}-\sqrt{125}}{\sqrt{m}-\sqrt{5}}\cdot\cfrac{1}{m-5}-\cfrac{2\sqrt{5}}{\sqrt{m}-\sqrt{5}}+\cfrac{\sqrt{5m}}{m-5}=[x=\sqrt{m},\ y=\sqrt{5}]=$\\$=
\cfrac{x^3-y^3}{x-y}\cdot\cfrac{1}{x^2-y^2}-\cfrac{2y}{x-y}+\cfrac{xy}{x^2-y^2}=
\cfrac{(x-y)(x^2+xy+y^2)}{x-y}\cdot\cfrac{1}{(x-y)(x+y)}-\cfrac{2y}{x-y}+\cfrac{xy}{(x-y)(x+y)}=
\cfrac{x^2+xy+y^2-2xy-2y^2+xy}{(x-y)(x+y)}=\cfrac{x^2-y^2}{(x-y)(x+y)}=\cfrac{(x-y)(x+y)}{(x-y)(x+y)}=1.$\\
22. $\cfrac{a\sqrt{a}+27}{a-3\sqrt{a}+9}-3=[x=\sqrt{a}]=\cfrac{x^3+27}{x^2-3x+9}-3=\cfrac{(x+3)(x^2-3x+9)}{x^2-3x+9}-3=x+3-3=x=\sqrt{a}.$\\
23. $\cfrac{a\sqrt{a}-27}{a+3\sqrt{a}+9}+3=[x=\sqrt{a}]=\cfrac{x^3-27}{x^2+3x+9}+3=\cfrac{(x-3)(x^2+3x+9)}{x^2+3x+9}+3=x-3+3=x=\sqrt{a}.$\\
24. $2a^3+3a^2-5=2a^3-2a^2+5a^2-5=2a^2(a-1)+5(a-1)(a+1)=(a-1)(2a^2+5a+5).$\\
25. $2a^3+3a-5=2a^3-2a+5a-5=2a(a-1)(a+1)+5(a-1)=(a-1)(2a^2+2a+5).$\\
26. $\cfrac{\cfrac{1}{a+b}-\cfrac{1}{a-b}}{\cfrac{1}{a+b}+\cfrac{1}{a-b}}\cdot\cfrac{a}{b}=\cfrac{\cfrac{a-b-a-b}{(a-b)(a+b)}}{\cfrac{a-b+a+b}{(a-b)(a+b)}}\cdot\cfrac{a}{b}=
\cfrac{\cfrac{-2b}{(a-b)(a+b)}}{\cfrac{2a}{(a-b)(a+b)}}\cdot\cfrac{a}{b}=-1.$\\
27. $\cfrac{\cfrac{1}{a-b}-\cfrac{1}{a+b}}{\cfrac{1}{a-b}+\cfrac{1}{a+b}}\cdot\cfrac{a}{b}=\cfrac{\cfrac{a+b-a+b}{(a-b)(a+b)}}{\cfrac{a+b+a-b}{(a-b)(a+b)}}\cdot\cfrac{a}{b}=
\cfrac{\cfrac{2b}{(a-b)(a+b)}}{\cfrac{2a}{(a-b)(a+b)}}\cdot\cfrac{a}{b}=1.$\\
28. $\cfrac{x^4+4}{(x+1)^2+1}=\cfrac{x^4+4x^2+4-4x^2}{x^2+2x+1+1}=\cfrac{(x^2+2)^2-(2x)^2}{x^2+2x+2}=\cfrac{(x^2-2x+2)(x^2+2x+2)}{x^2+2x+2}=x^2-2x+2.$\\
29. $\cfrac{x^4+4}{(x-1)^2+1}=\cfrac{x^4+4x^2+4-4x^2}{x^2-2x+1+1}=\cfrac{(x^2+2)^2-(2x)^2}{x^2-2x+2}=\cfrac{(x^2-2x+2)(x^2+2x+2)}{x^2-2x+2}=x^2+2x+2.$\\
30. $\sqrt{b-2+2\sqrt{b-3}}=\sqrt{(\sqrt{b-3})^2+2\sqrt{b-3}+1}=\sqrt{b-3}+1.$\\
31. $\sqrt{a-1+2\sqrt{a-2}}=\sqrt{(\sqrt{a-2})^2+2\sqrt{a-2}+1}=\sqrt{a-2}+1.$\\
32. $\cfrac{a^2}{(a+1)(a-c)}+\cfrac{1}{(c+1)(a+1)}+\cfrac{c^2}{(c-a)(c+1)}=\cfrac{a^2c+a^2+a-c-ac^2-c^2}{(a+1)(a-c)(c+1)}=$\\$=
\cfrac{ac(a-c)+(a-c)(a+c)+a-c}{(a+1)(a-c)(c+1)}=\cfrac{(a-c)(ac+a+c+1)}{(a+1)(a-c)(c+1)}=\cfrac{(a-c)(a+1)(c+1)}{(a+1)(a-c)(c+1)}=1.$\\
33. $\cfrac{9}{(b-3)(c-3)}-\cfrac{b^2}{(b-c)(3-b)}-\cfrac{c^2}{(3-c)(c-b)}=\cfrac{9b-9c+b^2c-3b^2-c^2b+3c^2}{(b-3)(c-3)(b-c)}=$\\$=
\cfrac{bc(b-c)-3(b-c)(b+c)+9(b-c)}{(b-3)(c-3)(b-c)}=\cfrac{(b-c)(bc-3b-3c+9)}{(b-3)(c-3)(b-c)}=\cfrac{(b-3)(c-3)(b-c)}{(b-3)(c-3)(b-c)}=1.$\\
34. $\cfrac{a^2-4b^2}{0,5a-b}-4b=\cfrac{(a-2b)(a+2b)}{0,5(a-2b)}-4b=2a+4b-4b=2a.$\\
35. $\cfrac{4a^2-b^2}{a-0,5b}-4a=\cfrac{(2a-b)(2a+b)}{0,5(2a-b)}-4a=4a+2b-4a=2b.$\\
36. $a^3-2a+1=a(a-1)(a+1)-(a-1)=(a-1)(a^2+a-1).$\\
37. $a^3-2a-1=a(a-1)(a+1)-(a+1)=(a+1)(a^2-a-1).$\\
38. $\cfrac{x}{a}-\cfrac{x^2-a^2}{a^2}\cdot\cfrac{a}{x+a}=\cfrac{x}{a}-\cfrac{(x-a)(x+a)}{a^2}\cdot\cfrac{a}{x+a}=\cfrac{x}{a}-\cfrac{x-a}{a}=\cfrac{a}{a}=1.$\\
39. $\cfrac{b^2-c^2}{c^2}\cdot\cfrac{c}{b-c}-\cfrac{b}{c}=\cfrac{(b-c)(b+c)}{c^2}\cdot\cfrac{c}{b-c}-\cfrac{b}{c}=\cfrac{b+c}{c}-\cfrac{b}{c}=\cfrac{c}{c}=1.$\\
40. $3x^2-11xy-4y^2=3x(x-4y)+y(x-4y)=(3x+y)(x-4y).$\\
41. $6y^2+11xy-2x^2=6y(y+2x)-x(y+2x)=(6y-x)(2x+y).$\\
42. $\cfrac{x^3+5x^2+3x-9}{x^2+6x+9}=\cfrac{x^2(x+3)+2x(x+3)-3(x+3)}{(x+3)^2}=\cfrac{(x+3)(x^2+2x-3)}{(x+3)^2}=\cfrac{(x+3)(x-1)}{x+3}=x-1.$\\
43. $\cfrac{x^3-2x^2-5x+6}{x^2-4x+3}=\cfrac{x^2(x-1)-x(x-1)-6(x-1)}{(x-3)(x-1)}=\cfrac{(x-1)(x^2-x-6)}{(x-3)(x-1)}=\cfrac{(x-3)(x+2)}{x-3}=x+2.$\\
44. $\cfrac{a\sqrt{a}-1}{a+\sqrt{a}-2}+\cfrac{3(\sqrt{a}+1)}{\sqrt{a}+2}=[x=\sqrt{a}]=
\cfrac{x^3-1}{x^2+x-2}+\cfrac{3(x+1)}{x+2}=\cfrac{(x-1)(x^2+x+1)}{(x+2)(x-1)}+\cfrac{3(x+1)}{x+2}=\cfrac{x^2+x+1}{x+2}+\cfrac{3(x+1)}{x+2}=
\cfrac{x^2+4x+4}{x+2}=\cfrac{(x+2)^2}{x+2}=x+2=\sqrt{a}+2.$\\
45. $\cfrac{a\sqrt{a}+1}{a-\sqrt{a}-2}-\cfrac{3(\sqrt{a}-1)}{\sqrt{a}-2}=[x=\sqrt{a}]=
\cfrac{x^3+1}{x^2-x-2}-\cfrac{3(x-1)}{x-2}=\cfrac{(x+1)(x^2-x+1)}{(x-2)(x+1)}-\cfrac{3(x-1)}{x-2}=
\cfrac{x^2-x+1}{x-2}-\cfrac{3(x-1)}{x-2}=\cfrac{x^2-4x+4}{x-2}=\cfrac{(x-2)^2}{x-2}=x-2=\sqrt{a}-2.$\\
46. $\sqrt{t^2+\cfrac{9}{t^2}+6}=\sqrt{t^2+2\cdot t\cdot\cfrac{3}{t}+\cfrac{9}{t^2}}=\sqrt{\left(t+\cfrac{3}{t}
ight)^2}=\left|t+\cfrac{3}{t}
ight|=\left|-0,5-6
ight|=6,5.$\\
47. $\sqrt{t^2+\cfrac{4}{t^2}+4}=\sqrt{t^2+2\cdot t\cdot\cfrac{2}{t}+\cfrac{4}{t^2}}=\sqrt{\left(t+\cfrac{2}{t}
ight)^2}=\left|t+\cfrac{2}{t}
ight|=\left|-0,5-4
ight|=4,5.$\\
48. $\left(\sqrt{m}+\cfrac{n}{\sqrt{m}+\sqrt{n}}
ight)\left(1+\cfrac{\sqrt{n^3}}{m\sqrt{m}-n\sqrt{n}}
ight)(
\sqrt{m}-\sqrt{n})=[x=\sqrt{m},\ y=\sqrt{n}]=$\\$=\left(x+\cfrac{y^2}{x+y}
ight)\left(1+\cfrac{y^3}{x^3-y^3}
ight)(
x-y)=\cfrac{x^2+xy+y^2}{x+y}\cdot\cfrac{x^3-y^3+y^3}{(x-y)(x^2+xy+y^2)}\cdot(x-y)=\cfrac{x^3}{x+y}=\cfrac{m\sqrt{m}}{\sqrt{m}+\sqrt{n}}.$\\
49. $a^2-9b^2+12bc-4c^2=a^2-(9b^2-12bc+4c^2)=a^2-(3b-2c)^2=(a+3b-2c)(a-3b+2c).$\\
50. $a^2-4b^2+12bc-9c^2=a^2-(4b^2-12bc+9c^2)=a^2-(2b-3c)^2=(a+2b-3c)(a-2b+3c).$\\
51. $\cfrac{2\sqrt{x}+x-x\sqrt{x}}{x-2\sqrt{x}}=[a=\sqrt{x}]=
\cfrac{2a+a^2-a^3}{a^2-2a}=\cfrac{(-a)(a^2-a-2)}{a(a-2)}=\cfrac{(-a)(a-2)(a+1)}{a(a-2)}=-a-1=-\sqrt{x}-1.$\\
52. $\cfrac{3\sqrt{x}-2x-x\sqrt{x}}{x+3\sqrt{x}}=[a=\sqrt{x}]=
\cfrac{3a-2a^2-a^3}{a^2+3a}=\cfrac{(-a)(a^2+2a-3)}{a(a+3)}=\cfrac{(-a)(a-1)(a+3)}{a(a+3)}=-a+1=1-\sqrt{x}.$\\
53. $x^3+4x^2+x-6=x^3-1+4(x^2-1)+x-1=(x-1)(x^2+x+1)+4(x-1)(x+1)+x-1=(x-1)(x^2+x+1+4x+4+1)=(x-1)(x^2+5x+6)=(x-1)(x+2)(x+3).$\\
54. $x^3-4x^2+x+6=x^3+1-4(x^2-1)+x+1=(x+1)(x^2-x+1)-4(x-1)(x+1)+x+1=(x+1)(x^2-x+1-4x+4+1)=(x+1)(x^2-5x+6)=(x+1)(x-2)(x-3).$\\
55. $\left(c-\cfrac{c^3+8}{2c+c^2}
ight)\cdot\cfrac{c}{c^2-4c+4}+\cfrac{2}{2-c}=
\left(c-\cfrac{(c+2)(c^2-2c+4)}{c(c+2)}
ight)\cdot\cfrac{c}{(c-2)^2}+\cfrac{2}{2-c}=
\cfrac{2(c-2)}{c}\cdot\cfrac{c}{(c-2)^2}+$\\$+\cfrac{2}{2-c}=\cfrac{2}{c-2}+\cfrac{2}{2-c}=0.$\\
56. $\left(c+\cfrac{8-c^3}{c^2-2c}
ight)\cdot\cfrac{c}{c^2+4c+4}+\cfrac{2}{2+c}=
\left(c+\cfrac{(2-c)(4+2c+c^2)}{c(c-2)}
ight)\cdot\cfrac{c}{(c+2)^2}+\cfrac{2}{2+c}=$\\$=
\cfrac{-2(c+2)}{c}\cdot\cfrac{c}{(c+2)^2}+\cfrac{2}{2+c}=\cfrac{-2}{c+2}+\cfrac{2}{2+c}=0.$\\
57. $9-x(x-y-3)+3(x-3-y)-y(3+y-x)=9-x(x-y-3)+3(x-y-3)+y(x-y-3)=9-(x-y-3)(x-y-3)=9-(x-y-3)^2=(3-x+y+3)(3+x-y-3)=(x-y)(y-x+6).$\\
58. $4-2(2-b-a)+a(2-a-b)-b(a+b-2)=4+2(a+b-2)-a(a+b-2)-b(a+b-2)=4-(a+b-2)(a+b-2)=4-(a+b-2)^2=(2-a-b+2)(2+a+b-2)=(a+b)(4-a-b).$\\
59. $\cfrac{x\sqrt{x}-y\sqrt{y}}{\sqrt{x}-\sqrt{y}}=[a=\sqrt{x},\ b=\sqrt{y}]=
\cfrac{a^3-b^3}{a-b}=\cfrac{(a-b)(a^2+ab+b^2)}{a-b}=a^2+ab+b^2=x+\sqrt{xy}+y.$\\
60. $\cfrac{x\sqrt{x}+y\sqrt{y}}{\sqrt{x}+\sqrt{y}}=[a=\sqrt{x},\ b=\sqrt{y}]=
\cfrac{a^3+b^3}{a+b}=\cfrac{(a+b)(a^2-ab+b^2)}{a+b}=a^2-ab+b^2=x-\sqrt{xy}+y.$\\
61. $\cfrac{a^2-1}{3a^2-4a+1}\cdot\cfrac{3a-1}{a}-\cfrac{1}{a}=
\cfrac{(a-1)(a+1)}{(3a-1)(a-1)}\cdot\cfrac{3a-1}{a}-\cfrac{1}{a}=\cfrac{a+1}{a}-\cfrac{1}{a}=\cfrac{a}{a}=1.$\\
62. $\cfrac{a^2-1}{4a^2-5a+1}\cdot\cfrac{4a-1}{a}-\cfrac{1}{a}=
\cfrac{(a-1)(a+1)}{(4a-1)(a-1)}\cdot\cfrac{4a-1}{a}-\cfrac{1}{a}=\cfrac{a+1}{a}-\cfrac{1}{a}=\cfrac{a}{a}=1.$\\
63. $\sqrt{xy}\left(\cfrac{x}{y}\sqrt{xy}-2\sqrt{\frac{x}{y}}+\sqrt{\frac{1}{xy}}
ight)=[a=\sqrt{x},\ b=\sqrt{y}]=
ab\left(\cfrac{a^2}{b^2}ab-2\cfrac{a}{b}+\cfrac{1}{ab}
ight)=ab\cdot\cfrac{a^4-2a^2+1}{ab}=(a^2-1)^2=(x-1)^2.$\\
64. $\cfrac{36+x}{6-\sqrt{-x}}=[a=\sqrt{-x}]=\cfrac{36-a^2}{6-a}=\cfrac{(6-a)(6+a)}{6-a}=a+6=\sqrt{-x}+6.$\\
65. $\cfrac{49x+1}{1+7\sqrt{-x}}=[a=\sqrt{-x}]=\cfrac{1-49a^2}{1+7a}=\cfrac{(1-7a)(1+7a)}{1+7a}=1-7a=1-7\sqrt{-x}.$\\
66. $1+4a^2b^2-(a^2+b^2)^2=1+4a^2b^2-a^4-2a^2b^2-b^4=1-(a^4-2a^2b^2+b^4)=1-(a^2-b^2)^2=(b^2+1-a^2)(a^2-b^2+1).$\\
67. $4x^2y^2-(x^2+y^2)^2+1=4x^2y^2-x^4-2x^2y^2-y^4+1=1-(x^4-2x^2y^2+y^4)=1-(x^2-y^2)^2=(y^2+1-x^2)(x^2-y^2+1).$\\
68. $\left(\sqrt{ab}+\cfrac{a\sqrt{a}-b\sqrt{b}}{\sqrt{a}-\sqrt{b}}
ight)\cdot\cfrac{a-\sqrt{ab}}{
a\sqrt{a}-b\sqrt{a}}=[x=\sqrt{a},\ y=\sqrt{b}]=
\left(xy+\cfrac{x^3-y^3}{x-y}
ight)\cdot\cfrac{x^2-xy}{
x^3-xy^2}=$\\$=\left(xy+\cfrac{(x-y)(x^2+xy+y^2)}{x-y}
ight)\cdot\cfrac{x(x-y)}{x(x-y)(x+y)}=
(x+y)^2\cdot\cfrac{1}{x+y}=x+y=\sqrt{a}+\sqrt{b}.$\\
69. $\left(\cfrac{x\sqrt{x}-8}{x-3\sqrt{x}+2}-\cfrac{6\sqrt{x}}{\sqrt{x}-1}
ight):
\left(1-\cfrac{1}{\sqrt{x}-1}
ight)=[a=\sqrt{x}]=
\left(\cfrac{a^3-8}{a^2-3a+2}-\cfrac{6a}{a-1}
ight):
\left(1-\cfrac{1}{a-1}
ight)=\left(\cfrac{(a-2)(a^2+2a+4)}{(a-2)(a-1)}-\cfrac{6a}{a-1}
ight):\cfrac{a-2}{a-1}=
\cfrac{(a-2)^2}{a-1}\cdot\cfrac{a-1}{a-2}=a-2=\sqrt{x}-2.$\\
70. $\left(\cfrac{1-x\sqrt{x}}{1+x+\sqrt{x}}+\sqrt{x}
ight): \cfrac{1+\sqrt{x}}{1-x}=[a=\sqrt{x}]=
\left(\cfrac{1-a^3}{1+a^2+a}+a
ight): \cfrac{1+a}{1-a^2}=$\\$=\left(\cfrac{(1-a)(1+a+a^2)}{1+a^2+a}+a
ight): \cfrac{1+a}{(1-a)(1+a)}=
1\cdot(1-a)=1-a=1-\sqrt{x}.$\\
71. $\left(\cfrac{a^3-8}{a^2-4}-\cfrac{6a}{a+2}
ight): \left(1-\cfrac{4}{a+2}
ight)^2=
\left(\cfrac{(a-2)(a^2+2a+4)}{(a-2)(a+2)}-\cfrac{6a}{a+2}
ight): \left(\cfrac{a-2}{a+2}
ight)^2=
\cfrac{(a-2)^2}{a+2}\cdot\cfrac{(a+2)^2}{(a-2)^2}=a+2.$\\
72. $\cfrac{b^2-1}{3b^2-4b+1}\cdot\cfrac{3b-1}{b}-\cfrac{1}{b}=
\cfrac{(b-1)(b+1)}{(3b-1)(b-1)}\cdot\cfrac{3b-1}{b}-\cfrac{1}{b}=\cfrac{b+1}{b}-\cfrac{1}{b}=\cfrac{b}{b}=1.$\\
73. $\cfrac{\sqrt{-ab^2}-\sqrt{a^2b}}{ab}-\cfrac{1}{\sqrt{b}}=[x=\sqrt{-a},\ y=\sqrt{b}]=
\cfrac{xy^2-x^2y}{-x^2y^2}-\cfrac{1}{y}=\cfrac{xy(y-x)}{-x^2y^2}-\cfrac{1}{y}=\cfrac{x-y}{xy}-\cfrac{1}{y}=-\cfrac{1}{x}=-\cfrac{1}{\sqrt{-a}}.$\\
74. $\cfrac{\sqrt{x}+1}{x\sqrt{x}+x+\sqrt{x}}:\cfrac{1}{x^2-\sqrt{x}}=[a=\sqrt{x}]=
\cfrac{a+1}{a^3+a^2+a}:\cfrac{1}{a^4-a}=\cfrac{a+1}{a(a^2+a+1)}\cdot a(a-1)(a^2+a+1)=a^2-1=x-1.$\\
75. $\cfrac{1}{x^2}\cdot\left(\cfrac{1}{(x-y)^2}+\cfrac{1}{y^2}
ight)+\cfrac{2}{x^3}\cdot\left(
\cfrac{1}{x-y}+\cfrac{1}{y}
ight)-\cfrac{1}{(x-y)^2y^2}=
\cfrac{1}{x^2}\cdot\cfrac{y^2+x^2-2xy+y^2}{(x-y)^2y^2}+\cfrac{2}{x^3}\cdot\cfrac{y+x-y}{(x-y)y}-\cfrac{1}{(x-y)^2y^2}=
\cfrac{x^2+2y^2-2xy}{x^2(x-y)^2y^2}+\cfrac{2}{x^2(x-y)y}-\cfrac{1}{(x-y)^2y^2}=\cfrac{2y(y-x)}{x^2(x-y)^2y^2}+\cfrac{2}{x^2(x-y)y}=
\cfrac{2}{x^2(x-y)y}-\cfrac{2}{x^2(x-y)y}=0.$\\
76. $\left(\sqrt{\sqrt{7}-\sqrt{5-a}}
ight)\cdot\sqrt{2+a}\cdot\left(\sqrt{\sqrt{7}+\sqrt{5-a}}
ight)-a=
\sqrt{2+a}\cdot\sqrt{7-(5-a)}-a=\sqrt{2+a}\cdot\sqrt{a+2}-a=a+2-a=2.$\\
77. $\left(\sqrt{\sqrt{5}-\sqrt{3-a}}
ight)\cdot\sqrt{2+a}\cdot\left(\sqrt{\sqrt{5}+\sqrt{3-a}}
ight)-a=
\sqrt{2+a}\cdot\sqrt{5-(3-a)}-a=\sqrt{2+a}\cdot\sqrt{2+a}-a=a+2-a=2.$\\
78. $\sqrt{a^2-4a+4}+\sqrt{a^2-12a+36}=\sqrt{(a-2)^2}+\sqrt{(a-6)^2}=|a-2|+|a-6|.$\\
а) $\left|-\cfrac{2}{7}-2
ight|+\left|-\cfrac{2}{7}-6
ight|=2+\cfrac{2}{7}+6+\cfrac{2}{7}=\cfrac{60}{7}.$\\
б) $|\sqrt{3+\sqrt{2}}-2|+|\sqrt{3+\sqrt{2}}-6|=\sqrt{3+\sqrt{2}}-2+6-\sqrt{3+\sqrt{2}}=4.$\\
79. $\sqrt{a^2-2a+1}+\sqrt{a^2-8a+16}=\sqrt{(a-1)^2}+\sqrt{(a-4)^2}=|a-1|+|a-4|.$\\
а) $\left|\cfrac{2}{7}-1
ight|+\left|\cfrac{2}{7}-4
ight|=1-\cfrac{2}{7}+4-\cfrac{2}{7}=\cfrac{31}{7}.$\\
б) $|\sqrt{3-\sqrt{2}}-1|+|\sqrt{3-\sqrt{2}}-4|=\sqrt{3-\sqrt{2}}-1+4-\sqrt{3-\sqrt{2}}=3.$\\
80. $x^4+64=x^4+16x^2+64-16x^2=(x^2+8)^2-(4x)^2=(x^2-4x+8)(x^2+4x+8).$\\
81. $\left(\cfrac{a\sqrt{a}+b\sqrt{b}}{\sqrt{a}+\sqrt{b}}-\sqrt{ab}
ight):(a-b)+\cfrac{2\sqrt{b}}{\sqrt{a}+\sqrt{b}}=[x=\sqrt{a},\ y=\sqrt{b}]=
\left(\cfrac{x^3+y^3}{x+y}-xy
ight):(x^2-y^2)+\cfrac{2y}{x+y}=\left(\cfrac{(x+y)(x^2-xy+y^2)}{x+y}-xy
ight):((x-y)(x+y))+\cfrac{2y}{x+y}=
(x-y)^2:((x-y)(x+y))+\cfrac{2y}{x+y}=\cfrac{x-y}{x+y}+\cfrac{2y}{x+y}=1.$\\
82. $36a^2-b^2+24bc-144c^2=36a^2-(b^2-24bc+144c^2)=36a^2-(b-12c)^2=(6a+b-12c)(6a-b+12c).$\\
83. $49m^2-121n^2+22nk-k^2=49m^2-(121n^2-22nk+k^2)=49m^2-(11n-k)^2=(7m-k+11n)(7m+k-11n).$\\
84. $\cfrac{6y-x}{x-2y}:\left(\cfrac{1}{x-2y}+\cfrac{1}{x-3y}-\cfrac{x+y}{x^2-5xy+6y^2}
ight)=
\cfrac{6y-x}{x-2y}:\left(\cfrac{1}{x-2y}+\cfrac{1}{x-3y}-\cfrac{x+y}{(x-2y)(x-3y)}
ight)=
\cfrac{6y-x}{x-2y}:\cfrac{x-3y+x-2y-x-y}{(x-2y)(x-3y)}=\cfrac{6y-x}{x-2y}\cdot\cfrac{(x-2y)(x-3y)}{x-6y}=3y-x.$\\
85. $\cfrac{3y-2x}{2x+y}:\left(\cfrac{1}{2x+y}-\cfrac{1}{3x-y}+\cfrac{x-y}{6x^2+xy-y^2}
ight)=
\cfrac{3y-2x}{2x+y}:\left(\cfrac{1}{2x+y}-\cfrac{1}{3x-y}+\cfrac{x-y}{(2x+y)(3x-y)}
ight)=
\cfrac{3y-2x}{2x+y}:\cfrac{3x-y-2x-y+x-y}{(2x+y)(3x-y)}=\cfrac{3y-2x}{2x+y}\cdot\cfrac{(2x+y)(3x-y)}{2x-3y}=y-3x.$\\
86. $\left(\cfrac{\sqrt{b}}{\sqrt{a}-\sqrt{b}}-\cfrac{\sqrt{b}}{\sqrt{a}+\sqrt{b}}
ight)\cdot\cfrac{\sqrt{a}+\sqrt{b}}{2b}=[x=\sqrt{a},\ y=\sqrt{b}]=
\left(\cfrac{y}{x-y}-\cfrac{y}{x+y}
ight)\cdot\cfrac{x+y}{2y^2}=$\\$
\cfrac{xy+y^2-xy+y^2}{(x-y)(x+y)}\cdot\cfrac{x+y}{2y^2}=\cfrac{1}{x-y}=\cfrac{1}{\sqrt{a}-\sqrt{b}}.$\\
87. $\left(\cfrac{\sqrt{a}}{\sqrt{a}-\sqrt{b}}+\cfrac{\sqrt{a}}{\sqrt{a}+\sqrt{b}}
ight)\cdot\cfrac{\sqrt{a}-\sqrt{b}}{2a}=[x=\sqrt{a},\ y=\sqrt{b}]=
\left(\cfrac{x}{x-y}+\cfrac{x}{x+y}
ight)\cdot\cfrac{x-y}{2x^2}=$\\$
\cfrac{x^2+xy+x^2-xy}{(x-y)(x+y)}\cdot\cfrac{x-y}{2x^2}=\cfrac{1}{x+y}=\cfrac{1}{\sqrt{a}+\sqrt{b}}.$\\
88. $x^2+2xy+y^2-z^2=(x+y)^2-z^2=(x+y-z)(x+y+z).$\\
89. $\cfrac{2^{n+2}+2^{n+2}}{3^{n+3}}=\cfrac{2\cdot2^{n+2}}{3^{n+3}}=\cfrac{2^{n+3}}{3^{n+3}}=\left(\cfrac{2}{3}
ight)^{n+3}.$\\
90. $\left(\cfrac{\sqrt{a}}{\sqrt{a}+\sqrt{b}}+\cfrac{\sqrt{b}}{\sqrt{a}-\sqrt{b}}+\cfrac{2\sqrt{ab}}{a-b}
ight)\left(\sqrt{a}-\cfrac{\sqrt{ab}+b}{\sqrt{a}+\sqrt{b}}
ight)=
[x=\sqrt{a},\ y=\sqrt{b}]=$\\$
\left(\cfrac{x}{x+y}+\cfrac{y}{x-y}+\cfrac{2xy}{x^2-y^2}
ight)\left(x-\cfrac{xy+y^2}{x+y}
ight)=
\cfrac{x^2-xy+xy+y^2+2xy}{(x-y)(x+y)}\cdot\left(x-\cfrac{y(x+y)}{x+y}
ight)=$\\$
\cfrac{(x+y)^2}{(x-y)(x+y)}\cdot\left(x-y
ight)=x+y=\sqrt{a}+\sqrt{b}.$\\
91. $a^3+a^2+2a-4=a^3-1+a^2-1+2a-2=(a-1)(a^2+a+1)+(a-1)(a+1)+2(a-1)=(a-1)(a^2+a+1+a+1+2)=(a-1)(a^2+2a+4).$\\
92. $\left(\cfrac{d-2}{d+2}-\cfrac{d^3+8}{d^2-4d+4}\cdot\cfrac{2-d}{d^2-2d+4}
ight):\left(d+2+\cfrac{8}{d-2}
ight)=$\\$
\left(\cfrac{d-2}{d+2}-\cfrac{(d+2)(d^2-2d+4)}{(d-2)^2}\cdot\cfrac{2-d}{d^2-2d+4}
ight):\cfrac{d^2-4+8}{d-2}=
\left(\cfrac{d-2}{d+2}+\cfrac{d+2}{d-2}
ight):\cfrac{d^2+4}{d-2}=$\\$
\cfrac{d^2-4d+4+d^2+4d+4}{(d-2)(d+2)}\cdot\cfrac{d-2}{d^2+4}=
\cfrac{2(d^2+4)}{d+2}\cdot\cfrac{1}{d^2+4}=\cfrac{2}{d+2}.$\\
93. $\left(\cfrac{c+2}{c-2}-\cfrac{8-c^3}{c^2+4c+4}\cdot\cfrac{c+2}{c^2+2c+4}
ight):\left(c-2+\cfrac{8}{c+2}
ight)=$\\$
\left(\cfrac{c+2}{c-2}-\cfrac{(2-c)(4+2c+c^2)}{(c+2)^2}\cdot\cfrac{c+2}{c^2+2c+4}
ight):\cfrac{c^2-4+8}{c+2}=
\left(\cfrac{c+2}{c-2}+\cfrac{c-2}{c+2}
ight)\cdot\cfrac{c+2}{c^2+4}=$\\$
\cfrac{c^2+4c+4+c^2-4c+4}{(c-2)(c+2)}\cdot\cfrac{c+2}{c^2+4}=
\cfrac{2(c^2+4)}{c-2}\cdot\cfrac{1}{c^2+4}=\cfrac{2}{c-2}.$\\
94. а) $T=\left(\cfrac{4}{2\sqrt{a}-3\sqrt{b}}-\cfrac{14\sqrt{b}}{2a+\sqrt{ab}-6b}+\cfrac{7}{\sqrt{a}+2\sqrt{b}}
ight):\left(\cfrac{1}{\sqrt{a}+2\sqrt{b}}-\cfrac{1}{\sqrt{a}}
ight)=
[x=\sqrt{a},\ y=\sqrt{b}]=
\left(\cfrac{4}{2x-3y}-\cfrac{14y}{2x^2+xy-6y^2}+\cfrac{7}{x+2y}
ight):\left(\cfrac{1}{x+2y}-\cfrac{1}{x}
ight)=$\\$
\left(\cfrac{4x+8y}{(2x-3y)(x+2y)}-\cfrac{14y}{(2x-3y)(x+2y)}+\cfrac{14x-21y}{(2x-3y)(x+2y)}
ight):\cfrac{x-x-2y}{x(x+2y)}=$\\$
\cfrac{18x-27y}{(2x-3y)(x+2y)}\cdot\cfrac{x(x+2y)}{-2y}=-\cfrac{9x}{2y}=-\cfrac{9\sqrt{a}}{2\sqrt{b}}.$\\
б) $x=\sqrt{92}=2\sqrt{23},\ y=\sqrt{207}=3\sqrt{23},$ тогда $T=-\cfrac{18\sqrt{2}}{6\sqrt{23}}=-3.$\\
в) $x=\sqrt{153}=3\sqrt{17},\ y=\sqrt{68}=2\sqrt{17},$ тогда $2x-3y=6\sqrt{17}-6\sqrt{17}=0,$ поэтому значение $T$ неопределено (присутствует деление на 0).\\
95. а) $M=\left(\cfrac{1}{\sqrt{c}+3\sqrt{d}}-\cfrac{1}{\sqrt{c}}
ight):\left(\cfrac{6}{3\sqrt{c}-2\sqrt{d}}-\cfrac{22\sqrt{d}}{3c+7\sqrt{cd}-6d}+\cfrac{3}{\sqrt{c}+3\sqrt{d}}
ight)=
[x=\sqrt{c},\ y=\sqrt{d}]=
\left(\cfrac{1}{x+3y}-\cfrac{1}{x}
ight):\left(\cfrac{6}{3x-2y}-\cfrac{22y}{3x^2+7xy-6y^2}+\cfrac{3}{x+3y}
ight)=$\\$
\cfrac{x-x-3y}{x(x+3y)}:\left(\cfrac{6x+18y}{(3x-2y)(x+3y)}-\cfrac{22y}{(3x-2y)(x+3y)}+\cfrac{9x-6y}{(3x-2y)(x+3y)}
ight)=$\\$
\cfrac{-3y}{x(x+3y)}:\cfrac{15x-10y}{(3x-2y)(x+3y)}=\cfrac{-3y}{x(x+3y)}\cdot\cfrac{(3x-2y)(x+3y)}{5(3x-2y)}=-\cfrac{3y}{5x}=-\cfrac{3\sqrt{d}}{5\sqrt{c}}.$\\
б) $x=\sqrt{99}=3\sqrt{11},\ y=\sqrt{275}=5\sqrt{11},$ тогда $M=-\cfrac{15\sqrt{11}}{15\sqrt{11}}=-1.$\\
в) $x=\sqrt{76}=2\sqrt{19},\ y=\sqrt{171}=3\sqrt{19},$ тогда $3x-2y=6\sqrt{19}-6\sqrt{19}=0,$ поэтому значение $M$ неопределено (присутствует деление на 0).\\
96. $\cfrac{x^2+x\sqrt{2}}{x^2+2}\left(\cfrac{x}{x-\sqrt{2}}-\cfrac{\sqrt{2}}{x+\sqrt{2}}
ight)=
\cfrac{x(x+\sqrt{2})}{x^2+2}\cdot\cfrac{x^2+x\sqrt{2}-x\sqrt{2}+2}{(x-\sqrt{2})(x+\sqrt{2})}=$\\$
\cfrac{x(x+\sqrt{2})}{x^2+2}\cdot\cfrac{x^2+2}{(x-\sqrt{2})(x+\sqrt{2})}=\cfrac{x}{x-\sqrt{2}}.$\\
97. $\left(\cfrac{\sqrt{a}}{\sqrt{a}-\sqrt{b}}-\cfrac{\sqrt{b}}{\sqrt{a}+\sqrt{b}}
ight)\cdot\cfrac{a-b}{a^2+ab}=
\cfrac{a+\sqrt{ab}-\sqrt{ab}+b}{a-b}\cdot\cfrac{a-b}{a(a+b)}=
\cfrac{a+b}{a-b}\cdot\cfrac{a-b}{a(a+b)}=\cfrac{1}{a}.$\\
98. $\left(\cfrac{\sqrt{a}-5}{\sqrt{a}+5}+\cfrac{20\sqrt{a}}{a-25}
ight):\cfrac{\sqrt{a}+5}{a-5\sqrt{a}}=[x=\sqrt{a}]=
\left(\cfrac{x-5}{x+5}+\cfrac{20x}{x^2-25}
ight):\cfrac{x+5}{x^2-5x}=$\\$
\left(\cfrac{x-5}{x+5}+\cfrac{20x}{(x-5)(x+5)}
ight)\cdot\cfrac{x(x-5)}{x+5}=\cfrac{x^2-10x+25+20x}{(x-5)(x+5)}\cdot\cfrac{x(x-5)}{x+5}=
\cfrac{(x+5)^2}{(x-5)(x+5)}\cdot\cfrac{x(x-5)}{x+5}=x=\sqrt{a}.$\\
99. $\left(\sqrt{ab}+\cfrac{a\sqrt{a}-b\sqrt{b}}{\sqrt{a}-\sqrt{b}}
ight)\cdot\cfrac{a-\sqrt{ab}}{a\sqrt{a}-b\sqrt{a}}=
[x=\sqrt{a}, y=\sqrt{b}]=\left(xy+\cfrac{x^3-y^3}{x-y}
ight)\cdot\cfrac{x^2-xy}{x^3-y^2x}=$\\$
\left(xy+\cfrac{(x-y)(x^2+xy+y^2)}{x-y}
ight)\cdot\cfrac{x(x-y)}{x(x-y)(x+y)}=
(x+y)^2\cdot\cfrac{1}{x+y}=x+y=\sqrt{a}+\sqrt{b}.$\\
100. $\left(1+\cfrac{\sqrt{xy}}{x+y+\sqrt{xy}}
ight)\cdot\cfrac{x\sqrt{x}-y\sqrt{y}}{y-x}=
[a=\sqrt{x},\ b=\sqrt{y}]=\left(1+\cfrac{ab}{a^2+b^2+ab}
ight)\cdot \cfrac{a^3-b^3}{b^2-a^2}=
\cfrac{(a+b)^2}{a^2+b^2+ab}\cdot \cfrac{(a-b)(a^2+ab+b^2)}{(b-a)(b+a)}=-a-b=-\sqrt{x}-\sqrt{y}.$\\
101. $\left(1-\cfrac{\sqrt{xy}}{x+y-\sqrt{xy}}
ight)\cdot\cfrac{x\sqrt{x}+y\sqrt{y}}{y-x}=
[a=\sqrt{x},\ b=\sqrt{y}]=\left(1-\cfrac{ab}{a^2+b^2-ab}
ight)\cdot \cfrac{a^3+b^3}{b^2-a^2}=
\cfrac{(a-b)^2}{a^2+b^2-ab}\cdot \cfrac{(a+b)(a^2-ab+b^2)}{(b-a)(b+a)}=b-a=\sqrt{y}-\sqrt{x}.$\\
102. $x^4+2x^3y-3x^2-2x-6xy-4y=x^3(x+2y)-3x(x+2y)-2(x+2y)=(x+2y)(x^3-3x-2)=
(x+2y)(x(x^2-1)-2(x+1))=(x+2y)(x(x-1)(x+1)-2(x+1))=
(x+2y)(x+1)(x^2-x-2)=(x+2y)(x+1)^2(x-2).$\\
103. $x^4-2x^3y-3x^2+6xy+2x-4y=x^3(x-2y)-3x(x-2y)+2(x-2y)=(x-2y)(x^3-3x+2)=
(x-2y)(x(x^2-1)-2(x-1))=(x-2y)(x(x-1)(x+1)-2(x-1))=
(x-2y)(x-1)(x^2+x-2)=(x-2y)(x-1)^2(x+2).$\\
104. $\left(\cfrac{1}{a+\sqrt{2}}-\cfrac{a^2+4}{a^3+2\sqrt{2}}
ight) \left (\cfrac{a-\sqrt{2}}{2}+\cfrac{1}{a}
ight)=[b=\sqrt{2}]=
\left(\cfrac{1}{a+b}-\cfrac{a^2+2b^2}{a^3+b^3}
ight) \left (\cfrac{a-b}{b^2}+\cfrac{1}{a}
ight)=$\\$\left(\cfrac{1}{a+b}-\cfrac{a^2+2b^2}{(a+b)(a^2-ab+b^2)}
ight) \cfrac{a^2-ab+b^2}{ab^2}=\cfrac{a^2-ab+b^2-a^2-2b^2}{(a+b)(a^2-ab+b^2)}\cdot
\cfrac{a^2-ab+b^2}{ab^2}=\cfrac{-b(a+b)}{(a+b)ab^2}=-\cfrac{1}{ab}=-\cfrac{1}{\sqrt{2}a}.$\\
105. $\left(\cfrac{1}{a-\sqrt{3}}-\cfrac{a^2+6}{a^3-3\sqrt{3}}
ight) \left (\cfrac{a+\sqrt{3}}{3}+\cfrac{1}{a}
ight)=[b=\sqrt{3}]=
\left(\cfrac{1}{a-b}-\cfrac{a^2+2b^2}{a^3-b^3}
ight) \left (\cfrac{a+b}{b^2}+\cfrac{1}{a}
ight)=$\\$\left(\cfrac{1}{a-b}-\cfrac{a^2+2b^2}{(a-b)(a^2+ab+b^2)}
ight) \cfrac{a^2+ab+b^2}{ab^2}=\cfrac{a^2+ab+b^2-a^2-2b^2}{(a-b)(a^2+ab+b^2)}\cdot
\cfrac{a^2+ab+b^2}{ab^2}=\cfrac{b(a-b)}{(a-b)ab^2}=\cfrac{1}{ab}=\cfrac{1}{\sqrt{3}a}.$

ewpage
