10. $\left(\cfrac{\sqrt{a}}{\sqrt{a}+\sqrt{b}}+\cfrac{\sqrt{b}}{\sqrt{a}-\sqrt{b}}+
\cfrac{2\sqrt{ab}}{a-b}
ight)\cdot\left(\sqrt{a}-\cfrac{\sqrt{ab}+b}{\sqrt{a}+\sqrt{b}}
ight)=[x=\sqrt{a},\ y=\sqrt{b}]=$\\$=
\left(\cfrac{x}{x+y}+\cfrac{y}{x-y}+
\cfrac{2xy}{x^2-y^2}
ight)\cdot\left(x-\cfrac{xy+y^2}{x+y}
ight)=\cfrac{x^2-xy+xy+y^2+2xy}{(x-y)(x+y)}\cdot\left(x-\cfrac{y(x+y)}{x+y}
ight)=$\\$=
\cfrac{x^2-xy+xy+y^2+2xy}{(x-y)(x+y)}\cdot(x-y)=\cfrac{x^2+2xy+y^2}{x+y}=\cfrac{(x+y)^2}{x+y}=x+y=\sqrt{a}+\sqrt{b}.$\\
