42. $\cfrac{44}{4-x^2}+\cfrac{2x+7}{x-2}=\cfrac{3-x}{x+2}\Big|\cdot(x-2)(x+2)\Leftrightarrow
\begin{cases} -44+(2x+7)(x+2)=(3-x)(x-2),\\ x\neq\pm2.\end{cases}\Leftrightarrow$\\$
\begin{cases}-44+2x^2+4x+7x+14=3x-6-x^2+2x,\\ x\neq\pm2.\end{cases}\Leftrightarrow
\begin{cases}3x^2+6x-24=0,\\ x\neq\pm2.\end{cases}\Leftrightarrow
\begin{cases}x^2+2x-8=0,\\ x\neq\pm2.\end{cases}\Leftrightarrow
\begin{cases}(x+1)^2-9=0,\\ x\neq\pm2.\end{cases}\Leftrightarrow
\begin{cases}(x-2)(x+4)=0,\\ x\neq\pm2.\end{cases}\Leftrightarrow
x=-4.$\\
