109. $\left(\cfrac{6x-1}{x^2+6x}+\cfrac{6x+1}{x^2-6x}\right):\cfrac{x^2+1}{x^2-36}-\cfrac{12}{x-1}=\cfrac{12}{x-x^2}\Leftrightarrow
\left(\cfrac{6x-1}{x(x+6)}+\cfrac{6x+1}{x(x-6)}\right)\cdot\cfrac{(x-6)(x+6)}{x^2+1}-\cfrac{12}{x-1}+\cfrac{12}{x(x-1)}=0\Leftrightarrow
\cfrac{6x^2-36x-x+6+6x^2+x+36x+6}{x(x-6)(x+6)}\cdot\cfrac{(x-6)(x+6)}{x^2+1}+\cfrac{12-12x}{x(x-1)}=0\Leftrightarrow
\cfrac{12(x^2+1)}{x(x-6)(x+6)}\cdot\cfrac{(x-6)(x+6)}{x^2+1}+\cfrac{12(1-x)}{x(x-1)}=0\Leftrightarrow
\begin{cases}
\cfrac{12}{x}-\cfrac{12}{x}=0,\\
x\neq\pm6, x\neq1.\end{cases}\Leftrightarrow x\notin\{-6;0;1;6\}$\\
