86. $a^2\left(1-\cfrac{1}{x}\right)-a\left(1+\cfrac{1}{x}\right)=\cfrac{a-3}{x}\Leftrightarrow
a^2-\cfrac{a^2}{x}-a-\cfrac{a}{x}-\cfrac{a-3}{x}=0\Leftrightarrow
\cfrac{-a^2-a-a+3}{x}=-a^2+a\Leftrightarrow
\cfrac{a^2+2a-3}{x}=a^2-a\Leftrightarrow
\cfrac{(a+1)^2-4}{x}=a(a-1)\Leftrightarrow
\cfrac{(a-1)(a+3)}{x}=a(a-1)\Leftrightarrow
\left[\begin{array}{l}\begin{cases} x\in\varnothing,\\ a\in\{-3;\ 0\}.\end{cases}\\
\begin{cases} x\neq0,\\ a=1.\end{cases}\\\begin{cases} x=\cfrac{a+3}{a},\\ a\notin\{-3;\ 0\ 1\}.\end{cases}\end{array}\right.$\\
