34. $\left(\cfrac{\sqrt[3]{\sqrt{3}+\sqrt{6}}\sqrt[6]{9-6\sqrt{2}}-\sqrt[6]{18}}{\sqrt[6]{2}-1}
ight)^3=
\left(\cfrac{\sqrt[6]{3+2\sqrt{18}+6}\sqrt[6]{9-6\sqrt{2}}-\sqrt[6]{2}\sqrt[6]{9}}{\sqrt[6]{2}-1}
ight)^3=$\\$
\left(\cfrac{\sqrt[6]{(9+6\sqrt{2})(9-6\sqrt{2})}-\sqrt[6]{2}\sqrt[6]{9}}{\sqrt[6]{2}-1}
ight)^3=
\left(\cfrac{\sqrt[6]{81-72}-\sqrt[6]{2}\sqrt[6]{9}}{\sqrt[6]{2}-1}
ight)^3=
\left(\cfrac{\sqrt[6]{9}(1-\sqrt[6]{2})}{\sqrt[6]{2}-1}
ight)^3=
\left(-\sqrt[6]{9}
ight)^3=-\sqrt{9}=-3.$\\
