95. $\cfrac{(4-x(2y+x)-y^2)}{(2x-2y+xy-4)(x^2+y^2-2(x+y-1))}=0\Leftrightarrow$\\$
\begin{cases}

4-x(2y+x)-y^2=0,\\
(2x-2y+xy-4)(x^2+y^2-2(x+y-1))
eq0.
\end{cases}\Leftrightarrow$\\$
\begin{cases}
4-2xy-x^2-y^2=0,\\
x^2+y^2-2x-2y+2
eq0,\\
x(y+2)-2(y+2)
eq0.
\end{cases}\Leftrightarrow
\begin{cases}
4=(y+x)^2,\\
(x-1)^2+(y-1)^2
eq0,\\
(x-2)(y+2)
eq0.
\end{cases}\Leftrightarrow
\begin{cases}
\left[\begin{array}{l}
y=2-x,\\
y=-2-x,
\end{array}
ight.\\
(x;y)
eq (1;1),\\
x
eq2,\\
y
eq-2.
\end{cases}$
\begin{figure}[ht!]
\center{\includegraphics[scale=0.35]{gr7-98.png}}
\end{figure}

ewpage
