43. $2x^2+3x-17=2(2-\sqrt{7})^2+3(2-\sqrt{7})-17\Leftrightarrow\begin{cases}2x^2+3x-17=2a^2+3a-17,\\ a=2-\sqrt{7}.\end{cases}
\Leftrightarrow$\\$\begin{cases}2(x-a)(x+a)+3(x-a)=0,\\ a=2-\sqrt{7}.\end{cases}
\Leftrightarrow\begin{cases}(x-a)(2x+2a+3)=0,\\ a=2-\sqrt{7}.\end{cases}
\Leftrightarrow \begin{cases}\left[\begin{gathered}
     x=a,\hfill\\
     x=\cfrac{-2a-3}{2}.\hfill \end{gathered}
ight.\\ a=2-\sqrt{7}.\end{cases}\Leftrightarrow$\\$
\left[\begin{gathered}
     x=2-\sqrt{7},\hfill\\
     x=\cfrac{2\sqrt{7}-7}{2}.\hfill \end{gathered}
ight.$\\
