92. $x^2-6x+7+\cfrac{2}{x^2-6x+10}=0\Leftrightarrow \begin{cases}t-3+\cfrac{2}{t}=0,\\ t=x^2-6x+10
eq0.\end{cases}\Leftrightarrow
\begin{cases}t^2-3t+2=0,\\ t=x^2-6x+10
eq0.\end{cases}\Leftrightarrow\left[\begin{gathered}
     x^2-6x+10=1,\hfill\\
     x^2-6x+10=2.\hfill \end{gathered}
ight.\Leftrightarrow\left[\begin{gathered}
     x^2-6x+9=0,\hfill\\
     x^2-6x+8=0.\hfill \end{gathered}
ight.\Leftrightarrow\left[\begin{gathered}
     (x-3)^2=0,\hfill\\
     (x-4)(x-2)=0.\hfill \end{gathered}
ight.\Leftrightarrow x\in\{2;3;4\}.$\\
