113. $|3x^2+18x-23|-|13-2x^2-12x|=-1\Leftrightarrow |3x^2+18x-23|=|2x^2+12x-13|-1\Leftrightarrow |3(x^2+6x)-23|=|2(x^2+6x)-13|-1.$ Пусть $x^2+6x=t,$ тогда $|3t-23|=|2t-13|-1\Leftrightarrow \left[\begin{array}{l}\begin{cases} 23-3t=13-2t-1,\\ t<\cfrac{13}{2}.\end{cases}\\ \begin{cases} 23-3t=2t-13-1,\\ \cfrac{13}{2}\leqslant t\leqslant\cfrac{23}{3}.\end{cases}\\ \begin{cases} 3t-23=2t-13-1,\\ \cfrac{23}{3}<t.\end{cases}\end{array}
ight.\Leftrightarrow \left[\begin{array}{l}\begin{cases} t=11\\ t<\cfrac{13}{2}.\end{cases}\\ \begin{cases} t=\cfrac{37}{5},\\ \cfrac{13}{2}\leqslant t\leqslant\cfrac{23}{3}.\end{cases}\\ \begin{cases} t=9,\\ \cfrac{23}{3}<t.\end{cases}\end{array}
ight.\Leftrightarrow
t\in\left\{\cfrac{37}{5};9
ight\}\Leftrightarrow
\left[\begin{array}{l}x^2+6x=\cfrac{37}{5},\\ x^2+6x=9.\end{array}
ight.\Leftrightarrow
\left[\begin{array}{l}5x^2+30x-37=0,\\ x^2+6x-9=0.\end{array}
ight.\Leftrightarrow$\\$
x\in\left\{-3\pm3\sqrt{2};\cfrac{-15\pm\sqrt{410}}{5}
ight\}.$\\
