17. $\cfrac{3}{x-2}-\cfrac{4}{x-1}=\cfrac{1}{x-4}-\cfrac{2}{x-3}\Leftrightarrow \cfrac{3x-3-4x+8}{(x-2)(x-1)}=\cfrac{x-3-2x+8}{(x-4)(x-3)}\Leftrightarrow$\\$
\cfrac{-x+5}{(x-2)(x-1)}=\cfrac{-x+5}{(x-4)(x-3)}\Leftrightarrow \begin{cases} \left[\begin{array}{l}-x+5=0,\\
(x-2)(x-1)=(x-4)(x-3).\end{array}
ight.\\ x
otin\{1;2;3;4\}\end{cases}\Leftrightarrow$\\$\begin{cases}\left[\begin{array}{l}x=5,\\
x^2-2x-x+2=x^2-4x-3x+12.\end{array}
ight.\\ x
otin\{1;2;3;4\}\end{cases}\Leftrightarrow \begin{cases} \left[\begin{array}{l}x=5,\\
x=\cfrac{5}{2}.\end{array}
ight.\\ x
otin\{1;2;3;4\}\end{cases}\Leftrightarrow\left[\begin{array}{l}x=5,\\
x=\cfrac{5}{2}.\end{array}
ight.$\\
