7. $\cfrac{3}{1+x+x^2}=3-x-x^2 \Leftrightarrow \begin{cases}
\cfrac{3}{1+t}=3-t,\\
t=x^2+x.\end{cases}\Leftrightarrow\begin{cases}
3=3-t+3t-t^2,\\
t=x^2+x.\end{cases}\Leftrightarrow\begin{cases}
t(t-2)=0,\\
t=x^2+x.\end{cases}\Leftrightarrow \left[
\begin{gathered}
x^2+x=0, \hfill
\\
x^2+x=2. \hfill
\\
\end{gathered}

ight.\Leftrightarrow \left[
\begin{gathered}
x(x+1)=0, \hfill
\\
(x+2)(x-1)=0. \hfill
\\
\end{gathered}

ight.\Leftrightarrow \left[
\begin{gathered}
x=0, \hfill
\\
x=-1, \hfill
\\
x=-2, \hfill
\\
x=1. \hfill
\end{gathered}

ight.\hfill$\\
