122. $\cfrac{6x}{x^3+4}+\cfrac{x}{x^3-3}=0,7x\Leftrightarrow
\left[\begin{array}{l}\cfrac{6}{x^3+4}+\cfrac{1}{x^3-3}=0,7,\\ x=0.\end{array}
ight.\Leftrightarrow
\left[\begin{array}{l}\cfrac{6x^3-18+x^3+4}{(x^3+4)(x^3-3)}=0,7,\\ x=0.\end{array}
ight.\Leftrightarrow$\\$
\left[\begin{array}{l}\cfrac{x^3-2}{(x^3+4)(x^3-3)}=0,1,\\ x=0.\end{array}
ight.\Leftrightarrow
\left[\begin{array}{l}\begin{cases} 10t-20=t^2-3t+4t-12,\\t=x^3.\end{cases}\\ x=0.\end{array}
ight.\Leftrightarrow
\left[\begin{array}{l}\begin{cases} t^2-9t+8=0,\\t=x^3.\end{cases}\\ x=0.\end{array}
ight.\Leftrightarrow$\\$
\left[\begin{array}{l}\begin{cases} (t-8)(t-1)=0,\\t=x^3.\end{cases}\\ x=0.\end{array}
ight.\Leftrightarrow
\left[\begin{array}{l}x=2,\\ x=1, \\ x=0.\end{array}
ight.$\\
