31. $|5x-x^2-6|=x^2-5x-6 \Leftrightarrow \begin{cases}\left[
      \begin{gathered} 5x-x^2-6=x^2-5x-6,\hfill\\
      5x-x^2-6=-x^2+5x+6.\hfill \end{gathered}
ight.\\
x^2-5x-6\geqslant0.\end{cases}\Leftrightarrow \begin{cases}\left[
      \begin{gathered} 2x(x-5)=0,\hfill\\
      -6=6.\hfill \end{gathered}
ight.\\
x^2-5x-6\geqslant0.\end{cases}\Leftrightarrow \begin{cases}\left[
      \begin{gathered} x=0,\hfill\\
      x=5.\hfill \end{gathered}
ight.\\
x^2-5x-6\geqslant0.\end{cases}\Leftrightarrow x\in\{\varnothing\}.$\\
