69. $\left((2-7x)^2-0,26
ight)^2-0,01=0\Leftrightarrow\left((2-7x)^2-0,26-0,1
ight)\left((2-7x)^2-0,26+0,1
ight)=0\Leftrightarrow$\\$
\left((2-7x)^2-0,36
ight)\left((2-7x)^2-0,16
ight)=0\Leftrightarrow$\\$
\left(2-7x-0,6
ight)\left(2-7x+0,6
ight)\left(2-7x-0,4
ight)\left(2-7x+0,4
ight)=0\Leftrightarrow$\\$
\left(1,4-7x
ight)\left(2,6-7x
ight)\left(1,6-7x
ight)\left(2,4-7x
ight)=0\Leftrightarrow
\left[\begin{array}{l}7x=1,4,\\ 7x=2,6,\\7x=1,6,\\7x=2,4.\end{array}
ight.\Leftrightarrow
\left[\begin{array}{l}x=\cfrac{1}{5},\\ x=\cfrac{13}{35},\\x=\cfrac{8}{35},\\x=\cfrac{12}{35}.\end{array}
ight.$\\
