111. $\cfrac{12}{x-x^2}+\cfrac{12}{x-1}=\left(\cfrac{6x-1}{x^2+6x}+\cfrac{6x+1}{x^2-6x}
ight):\cfrac{x^2+1}{x^2-36}\Leftrightarrow
\left(\cfrac{6x-1}{x(x+6)}+\cfrac{6x+1}{x(x-6)}
ight)\cdot\cfrac{(x-6)(x+6)}{x^2+1}-\cfrac{12}{x-1}+\cfrac{12}{x(x-1)}=0\Leftrightarrow
\cfrac{6x^2-36x-x+6+6x^2+x+36x+6}{x(x-6)(x+6)}\cdot\cfrac{(x-6)(x+6)}{x^2+1}+\cfrac{12-12x}{x(x-1)}=0\Leftrightarrow
\cfrac{12(x^2+1)}{x(x-6)(x+6)}\cdot\cfrac{(x-6)(x+6)}{x^2+1}+\cfrac{12(1-x)}{x(x-1)}=0\Leftrightarrow
\begin{cases}
\cfrac{12}{x}-\cfrac{12}{x}=0,\\
x
eq\pm6, x
eq1.\end{cases}\Leftrightarrow x
otin\{-6;0;1;6\}$\\
