44. $\cfrac{7}{x-2}=3+\cfrac{x^3+27}{(x+3)(x-2)}\Leftrightarrow \cfrac{7}{x-2}=3+\cfrac{(x+3)(x^2-3x+9)}{(x+3)(x-2)}\Leftrightarrow
\begin{cases}\cfrac{7}{x-2}=3+\cfrac{x^2-3x+9}{x-2},\\ x
eq-3.\end{cases}\Leftrightarrow
\begin{cases}\cfrac{7}{x-2}=\cfrac{3x-6+x^2-3x+9}{x-2},\\ x
eq-3.\end{cases}\Leftrightarrow
\begin{cases}\cfrac{7}{x-2}=\cfrac{x^2+3}{x-2},\\ x
eq-3.\end{cases}\Leftrightarrow
\begin{cases}x^2+3=7,\\ x
eq-3;\ 2.\end{cases}\Leftrightarrow
\begin{cases}x^2-4=0,\\ x
eq-3;\ 2.\end{cases}\Leftrightarrow
\begin{cases}(x-2)(x+2)=0,\\ x
eq-3;\ 2.\end{cases}\Leftrightarrow
x=-2.$\\
