45. $\cfrac{x^2-4x-8}{5x-x^2}=\cfrac{x^2-3x-7}{x(x-5)}\Leftrightarrow\cfrac{8+4x-x^2}{x(x-5)}=\cfrac{x^2-3x-7}{x(x-5)}\Leftrightarrow
\begin{cases} 8+4x-x^2=x^2-3x-7,\\ x
eq0;\ 5.\end{cases}\Leftrightarrow
\begin{cases} 2x^2-7x-15=0,\\ x
eq0;\ 5.\end{cases}\Leftrightarrow
\begin{cases} 4x^2-14x-30=0,\\ x
eq0;\ 5.\end{cases}\Leftrightarrow
\begin{cases} (2x-3,5)^2-42,25=0,\\ x
eq0;\ 5.\end{cases}\Leftrightarrow$\\$
\begin{cases} (2x-3,5-6,5)(2x-3,5+6,5)=0,\\ x
eq0;\ 5.\end{cases}\Leftrightarrow
\begin{cases} (2x-10)(2x+3)=0,\\ x
eq0;\ 5.\end{cases}\Leftrightarrow
x=-\cfrac{3}{2}.$\\
