64. $\left(\cfrac{4x-7}{0,2}+\cfrac{6x-3}{0,4}
ight)^2=\left(70-\cfrac{4x+1}{0,3}
ight)^2\Leftrightarrow
\left(\cfrac{8x-14+6x-3}{0,4}
ight)^2=\left(\cfrac{21-4x-1}{0,3}
ight)^2\Leftrightarrow$\\$
\left(\cfrac{14x-17}{0,4}
ight)^2=\left(\cfrac{20-4x}{0,3}
ight)^2\Leftrightarrow
\left(\cfrac{14x-17}{0,4}-\cfrac{20-4x}{0,3}
ight)\left(\cfrac{14x-17}{0,4}+\cfrac{20-4x}{0,3}
ight)=0\Leftrightarrow$\\
$(290x-655)(130x+145)=0\Leftrightarrow \left[\begin{array}{l}x=\cfrac{131}{58},\\ x=-\cfrac{29}{26}.\end{array}
ight.$\\
