\section{Преобразование буквенных выражений решения}
1. $\left(\left(\cfrac{\sqrt{a}+\sqrt{b}}{\sqrt[4]{a}-\sqrt[4]{b}}
ight)^{-1}-
\cfrac{2\sqrt[4]{ab}}{b^{\frac{3}{4}}-a^{\frac{1}{4}}b^{\frac{1}{2}}+
a^{\frac{1}{2}}b^{\frac{1}{4}}-a^{\frac{3}{4}}}
ight)^{-1}=[x=\sqrt[4]{a},\ y=\sqrt[4]{b}]=$\\$
\left(\cfrac{x-y}{x^2+y^2}-\cfrac{2xy}{y^3-xy^2+x^2y-x^3}
ight)^{-1}=
\left(\cfrac{x-y}{x^2+y^2}-\cfrac{2xy}{y^2(y-x)+x^2(y-x)}
ight)^{-1}=$\\$
\left(\cfrac{x-y}{x^2+y^2}-\cfrac{2xy}{(y-x)(x^2+y^2)}
ight)^{-1}=
\left(\cfrac{x-y}{x^2+y^2}+\cfrac{2xy}{(x-y)(x^2+y^2)}
ight)^{-1}=
\left(\cfrac{x^2-2xy+y^2+2xy}{(x-y)(x^2+y^2)}
ight)^{-1}=$\\$x-y=\sqrt[4]{a}-\sqrt[4]{b}.$\\
2. $a^{\frac{4}{3}}\cdot\left(\cfrac{3}{\sqrt[3]{a^2}-\sqrt[3]{a}+1}-
\cfrac{3}{a+1}+\cfrac{\sqrt[3]{a}-1}{\sqrt[3]{a^2}-1}
ight)^{-1}
\left(\cfrac{a^{-\frac{1}{3}}+1}{a^\frac{1}{3}}
ight)^2=[x=\sqrt[3]{a}]=$\\$
x^4\cdot\left(\cfrac{3}{x^2-x+1}-\cfrac{3}{x^3+1}+\cfrac{x-1}{x^2-1}
ight)^{-1}\left(\cfrac{\cfrac{1}{x}+1}{x}
ight)^2=$\\$
x^4\cdot\left(\cfrac{3}{x^2-x+1}-\cfrac{3}{(x+1)(x^2-x+1)}+\cfrac{1}{x+1}
ight)^{-1}\left(\cfrac{x+1}{x^2}
ight)^2=$\\$
x^4\cdot\left(\cfrac{3x+3-3+x^2-x+1}{(x+1)(x^2-x+1)}
ight)^{-1}\cfrac{(x+1)^2}{x^4}=
\left(\cfrac{(x+1)^2}{(x+1)(x^2-x+1)}
ight)^{-1}(x+1)^2=\cfrac{x^3+1}{(x+1)^2}(x+1)^2=x^3+1=a+1.$\\
3. $\left(\cfrac{n-m}{\sqrt{n}+\sqrt{m}}
ight)^2:\left(\cfrac{\sqrt{n^3}-\sqrt{m^3}}{\sqrt{n}-\sqrt{m}}-3\sqrt{mn}
ight)=
[x=\sqrt{n},\ y=\sqrt{m}]=\left(\cfrac{x^2-y^2}{x+y}
ight)^2:\left(\cfrac{x^3-y^3}{x-y}-3xy
ight)=
\left(x-y
ight)^2:\left(x^2+xy+y^2-3xy
ight)=(x-y)^2:(x-y)^2=1.$\\
4. $\left(\cfrac{\sqrt{a^3}-\sqrt{b^3}}{\sqrt{a}-\sqrt{b}}+\sqrt{ab}
ight)\left(\cfrac{\sqrt{a}-\sqrt{b}}{a-b}
ight)^2=[x=\sqrt{a},\ y=\sqrt{b}]=
\left(\cfrac{x^3-y^3}{x-y}+xy
ight)\left(\cfrac{x-y}{x^2-y^2}
ight)^2=(x^2+xy+y^2+xy)\left(\cfrac{1}{x+y}
ight)^2=
(x+y)^2\cfrac{1}{(x+y)^2}=1.$\\
5. $\left(\cfrac{\sqrt[4]{ab^3}-\sqrt[4]{a^3b}}{\sqrt{a}-\sqrt{b}}
ight)^{-2}\cdot\sqrt{1+\cfrac{a}{b}+2\sqrt{\cfrac{a}{b}}}=[x=\sqrt[4]{a},\ y=\sqrt[4]{b}]=
\left(\cfrac{xy^3-x^3y}{x^2-y^2}
ight)^{-2}\cdot\sqrt{1+\cfrac{x^4}{y^4}+2\cfrac{x^2}{y^2}}=
\left(\cfrac{-xy(x^2-y^2)}{x^2-y^2}
ight)^{-2}\cdot\sqrt{\left(1+\cfrac{x^2}{y^2}
ight)^2}=
\cfrac{1}{x^2y^2}\cdot\cfrac{x^2+y^2}{y^2}=\cfrac{x^2+y^2}{x^2y^4}=\cfrac{\sqrt{a}+\sqrt{b}}{b\sqrt{a}}.$\\
6. $\left((\sqrt[4]{a}-\sqrt[4]{b})^{-1}+(\sqrt[4]{a}+\sqrt[4]{b})^{-1}
ight)^{-2}:\cfrac{a-b}{4(\sqrt{a}+\sqrt{b})}=[x=\sqrt[4]{a},\ y=\sqrt[4]{b}]=
\left((x-y)^{-1}+(x+y)^{-1}
ight)^{-2}:\cfrac{x^4-y^4}{4(x^2+y^2)}=
\left(\cfrac{1}{x-y}+\cfrac{1}{x+y}
ight)^{-2}\cdot\cfrac{4(x^2+y^2)}{(x^2-y^2)(x^2+y^2)}=
\left(\cfrac{x+y+x-y}{(x-y)(x+y)}
ight)^{-2}\cdot\cfrac{4}{x^2-y^2}=
\cfrac{(x-y)^2(x+y)^2}{4x^2}\cdot\cfrac{4}{(x-y)(x+y)}=\cfrac{x^2-y^2}{x^2}=\cfrac{\sqrt{a}-\sqrt{b}}{\sqrt{a}}.$\\
7. $\left(\sqrt{y}-\cfrac{x}{\sqrt{y}}
ight):\left(\sqrt{\cfrac{x}{y}}-\sqrt{\cfrac{y}{x}}
ight)=[a=\sqrt{x},\ b=\sqrt{y}]=
\left(b-\cfrac{a^2}{b}
ight):\left(\cfrac{a}{b}-\cfrac{b}{a}
ight)=\cfrac{b^2-a^2}{b}:\cfrac{a^2-b^2}{ab}=-a=-\sqrt{x}.$\\
8. $\left(\cfrac{y}{\sqrt{x}}-\sqrt{x}
ight):\left(\sqrt{\cfrac{x}{y}}-\sqrt{\cfrac{y}{x}}
ight)=[a=\sqrt{x},\ b=\sqrt{y}]=
\left(\cfrac{b^2}{a}-a
ight):\left(\cfrac{a}{b}-\cfrac{b}{a}
ight)=
\cfrac{b^2-a^2}{a}:\cfrac{a^2-b^2}{ab}=-b=-\sqrt{y}.$\\
9. $\cfrac{\sqrt{a-2\sqrt{a-1}}}{1-\sqrt{a-1}}=\cfrac{\sqrt{a-1-2\sqrt{a-1}+1}}{1-\sqrt{a-1}}=\cfrac{\sqrt{(\sqrt{a-1}-1)^2}}{1-\sqrt{a-1}}=
\cfrac{\sqrt{a-1}-1}{1-\sqrt{a-1}}=-1.$\\
10. $\cfrac{\sqrt{a-2\sqrt{a-1}}}{1-\sqrt{a-1}}=\cfrac{\sqrt{a-1-2\sqrt{a-1}+1}}{1-\sqrt{a-1}}\cfrac{\sqrt{(\sqrt{a-1}-1)^2}}{1-\sqrt{a-1}}=
\cfrac{1-\sqrt{a-1}}{1-\sqrt{a-1}}=1.$\\
11. $\cfrac{x-y}{\sqrt{x}+\sqrt{y}}:\left(\left(x^\frac{1}{4}-y^\frac{1}{4}
ight)^{-1}+\left(x^\frac{1}{4}+y^\frac{1}{4}
ight)^{-1}
ight)^{-2}=[a=x^{\frac{1}{4}},\ b=y^\frac{1}{4}]=\cfrac{a^4-b^4}{a^2+b^2}:\left(\cfrac{1}{a-b}+\cfrac{1}{a+b}
ight)^{-2}=
(a^2-b^2)\cdot\left(\cfrac{a+b+a-b}{a^2-b^2}
ight)^{2}=(a^2-b^2)\cfrac{4a^2}{(a^2-b^2)^2}=\cfrac{4a^2}{a^2-b^2}=\cfrac{4\sqrt{x}}{\sqrt{x}-\sqrt{y}}.$\\
12. $\left(\cfrac{1}{\left(a^\frac{1}{2}+b^\frac{1}{2}
ight)^{-2}}-\left(\cfrac{\sqrt{a}-\sqrt{b}}{a^\frac{3}{2}-b^\frac{3}{2}}
ight)^{-1}
ight):\sqrt{ab}=
[a=x^{\frac{1}{2}},\ b=y^\frac{1}{2}]=\left(\cfrac{1}{\left(x+y
ight)^{-2}}-\left(\cfrac{x-y}{x^3-y^3}
ight)^{-1}
ight):(xy)=
\left(x^2+2xy+y^2-x^2-xy-y^2
ight):(xy)=1.$\\
13. $(1-a^2):\left(\left(\cfrac{1-a\sqrt{a}}{1-\sqrt{a}}+\sqrt{a}
ight)\cdot\left(\cfrac{1+a\sqrt{a}}{1+\sqrt{a}}-\sqrt{a}
ight)
ight)+1=[x=\sqrt{a}]=$\\$
(1-x^4):\left(\left(\cfrac{1-x^3}{1-x}+x
ight)\cdot\left(\cfrac{1+x^3}{1+x}-x
ight)
ight)+1=
(1-x^4):\left(\left(1+x+x^2+x
ight)\cdot\left(1-x+x^2-x
ight)
ight)+1=
(1-x^4):\left((1+x)^2\cdot(1-x)^2
ight)+1=(1+x^2)(1-x^2):(1-x^2)^2+1=\cfrac{1+x^2}{1-x^2}+1=\cfrac{2}{1-x^2}=\cfrac{2}{1-a}.$\\
14. $\cfrac{(\sqrt{x}-\sqrt{y})^3+\cfrac{2x^2}{\sqrt{x}}+y\sqrt{y}}{x\sqrt{x}+y\sqrt{y}}+\cfrac{3\sqrt{xy}-3y}{x-y}=[a=\sqrt{x},\ b=\sqrt{y}]=
\cfrac{(a-b)^3+\cfrac{2a^4}{a}+b^3}{a^3+b^3}+\cfrac{3ab-3b^2}{a^2-b^2}=
\cfrac{a^3-3a^2b+3ab^2-b^3+2a^3+b^3}{a^3+b^3}+\cfrac{3b(a-b)}{(a-b)(a+b)}=
\cfrac{3a(a^2-ab+b^2)}{(a+b)(a^2-ab+b^2)}+\cfrac{3b}{a+b}=\cfrac{3a+3b}{a+b}=3.$\\
15. $\left(\cfrac{27^\frac{1}{2}-a^{-\frac{3}{2}}}{3^\frac{1}{2}-a^{-\frac{1}{2}}}+3^{\frac{1}{2}} a^{-\frac{1}{2}}

ight):(3-a^{-1})-\cfrac{2a^{-\frac{1}{2}}}{3^\frac{1}{2}-a^{-\frac{1}{2}}}=[x=3^{\frac{1}{2}},\ y=a^{-\frac{1}{2}}]=
\left(\cfrac{x^3-y^3}{x-y}+xy
ight):(x^2-y^2)-\cfrac{2y}{x-y}=\cfrac{x^2+xy+y^2+xy}{(x-y)(x+y)}-\cfrac{2y}{x-y}=
\cfrac{(x+y)^2}{(x-y)(x+y)}-\cfrac{2y}{x-y}=\cfrac{x+y-2y}{x-y}=1.$\\
16. $\left(\cfrac{8^\frac{1}{2}+y^{-\frac{3}{2}}}{2^\frac{1}{2}+y^{- \frac{1}{2}}}-
2^\frac{1}{2}y^{-\frac{1}{2}}
ight):(2-y^{-1})+\cfrac{2y^{-\frac{1}{2}}}{2^\frac{1}{2}+y^{-\frac{1}{2}}}=[x=2^{\frac{1}{2}},\ z=y^{-\frac{1}{2}}]=
\left(\cfrac{x^3+z^3}{x+z}-xz
ight):(x^2-z^2)+\cfrac{2z}{x+z}=\cfrac{x^2-xz+z^2-xz}{(x-z)(x+z)}+\cfrac{2z}{x+z}=
\cfrac{(x-z)^2}{(x-z)(x+z)}+\cfrac{2z}{x+z}=\cfrac{x-z+2z}{x+z}=1.$\\
17. $\left(\cfrac{x-9}{x+3\sqrt{x}+9}\cdot\left(\cfrac{x^{0,5}+3}{x^{1,5}-27}
ight)^{-1}
ight)^{0,5}+x^{0,5}=[a=\sqrt{x}]=
\left(\cfrac{a^2-9}{a^2+3a+9}\cdot\left(\cfrac{a+3}{a^3-27}
ight)^{-1}
ight)^{0,5}+a=
\left(\cfrac{(a-3)(a+3)}{a^2+3a+9}\cdot\cfrac{(a-3)(a^2+3a+9)}{a+3}
ight)^{0,5}+a=((a-3)^2)^{0,5}+a=3-a+a=3.$\\
18. $\left(\cfrac{a^\frac{3}{2}-8}{a^\frac{1}{2}+2}\cdot\left(\cfrac{a+2\sqrt{a}+4}{a-4}
ight)^{-1}
ight)^\frac{1}{2}-a^\frac{1}{2}=[x=a^\frac{1}{2}]=
\left(\cfrac{x^3-8}{x+2}\cdot\left(\cfrac{x^2+2x+4}{x^2-4}
ight)^{-1}
ight)^\frac{1}{2}-x=$\\$
\left(\cfrac{(x-2)(x^2+2x+4)}{x+2}\cdot\cfrac{(x-2)(x+2)}{x^2+2x+4}
ight)^\frac{1}{2}-x=((x-2)^2)^\frac{1}{2}-x=x-2-x=-2.$\\
19. $\left(\cfrac{\sqrt{a}-2}{a+2\sqrt{a}}+\cfrac{\sqrt{a}+2}{a-2\sqrt{a}}
ight)\cdot
\cfrac{a^\frac{3}{2}}{a+4}-\cfrac{8}{a-4}=[x=\sqrt{a}]=
\left(\cfrac{x-2}{x^2+2x}+\cfrac{x+2}{x^2-2x}
ight)\cdot\cfrac{x^3}{x^2+4}-\cfrac{8}{x^2-4}=
\left(\cfrac{x-2}{x(x+2)}+\cfrac{x+2}{x(x-2)}
ight)\cdot\cfrac{x^3}{x^2+4}-\cfrac{8}{x^2-4}=
\cfrac{x^2-4x+4+x^2+4x+4}{x(x+2)(x-2)}\cdot\cfrac{x^3}{x^2+4}-\cfrac{8}{x^2-4}=
\cfrac{2(x^2+4)}{x(x+2)(x-2)}\cdot\cfrac{x^3}{x^2+4}-\cfrac{8}{x^2-4}=
\cfrac{2x^2}{(x+2)(x-2)}-\cfrac{8}{(x+2)(x-2)}=\cfrac{2x^2-8}{(x+2)(x-2)}=\cfrac{2(x-2)(x+2)}{(x+2)(x-2)}=2.$\\
20. $\left(\cfrac{\sqrt{x-1}}{\sqrt{x-1}+\sqrt{x+1}}+\cfrac{x-1}{\sqrt{x^2-1}-x+1}
ight)(x^2-1)^{-\frac{1}{2}}=[a=\sqrt{x-1},\ b=\sqrt{x+1}]=$\\$
\left(\cfrac{a}{a+b}+\cfrac{a^2}{ab-a^2}
ight)((ab)^2)^{-\frac{1}{2}}=\left(\cfrac{a}{a+b}+\cfrac{a^2}{a(b-a)}
ight):(ab)=
\cfrac{ba-a^2+a^2+ab}{b^2-a^2}:(ab)=\cfrac{2}{b^2-a^2}=$\\$\cfrac{2}{x+1-x+1}=1.$\\
21. $\left(\cfrac{a^2+4}{a^3+2\sqrt{2}}-\cfrac{1}{a+\sqrt{2}}
ight):\left(\cfrac{a^2}{\sqrt{2}}-a+\sqrt{2}
ight)^{-1}=[b=\sqrt{2}]=
\left(\cfrac{a^2+2b^2}{a^3+b^3}-\cfrac{1}{a+b}
ight):\left(\cfrac{a^2}{b}-a+b
ight)^{-1}=
\left(\cfrac{a^2+2b^2}{(a+b)(a^2-ab+b^2)}-\cfrac{1}{a+b}
ight):\left(\cfrac{a^2-ab+b^2}{b}
ight)^{-1}=
\cfrac{a^2+2b^2-a^2+ab-b^2}{(a+b)(a^2-ab+b^2)}\cdot\cfrac{a^2-ab+b^2}{b}=$\\$\cfrac{b(a+b)}{(a+b)b}=1.$\\
22. $\left(\cfrac{a^\frac{3}{2}+1}{a-1}-\cfrac{a}{\sqrt{a}+1}-\cfrac{1}{\sqrt{a}-1}
ight)\cdot\left(\cfrac{1}{1+a^{-\frac{1}{2}}}
ight)^{-1}=[x=a^\frac{1}{2}]=
\left(\cfrac{x^3+1}{x^2-1}-\cfrac{x^2}{x+1}-\cfrac{1}{x-1}
ight)\cdot\left(\cfrac{1}{1+\cfrac{1}{x}}
ight)^{-1}$\\$=
\cfrac{x^3+1-x^3+x^2-x-1}{(x-1)(x+1)}\cdot\left(\cfrac{x}{x+1}
ight)^{-1}=
\cfrac{x(x-1)}{(x-1)(x+1)}\cdot\cfrac{x+1}{x}=1.$\\
23. $\left(\cfrac{\sqrt{x}-\sqrt{y}}{x\sqrt{y}+\sqrt{x}y}+\cfrac{\sqrt{x}+\sqrt{y}}{x\sqrt{y}-\sqrt{x}y}
ight)
\cdot\cfrac{\sqrt{x^3}\sqrt{y}}{x+y}=[a=\sqrt{x},\ b=\sqrt{y}]=
\left(\cfrac{a-b}{a^2b+ab^2}+\cfrac{a+b}{a^2b-ab^2}
ight)\cdot\cfrac{a^3b}{a^2+b^2}=
\left(\cfrac{a-b}{ab(a+b)}+\cfrac{a+b}{ab(a-b)}
ight)\cdot\cfrac{a^3b}{a^2+b^2}=
\cfrac{a^2-2ab+b^2+a^2+2ab+b^2}{ab(a-b)(a+b)}\cdot\cfrac{a^3b}{a^2+b^2}=
\cfrac{2(a^2+b^2)}{ab(a-b)(a+b)}\cdot\cfrac{a^3b}{a^2+b^2}=\cfrac{2a^2}{a^2-b^2}=\cfrac{2x}{x-y}.$\\
24. $\cfrac{m-n}{\sqrt{m}(\sqrt[4]{m}-\sqrt[4]{n})}-\cfrac{\sqrt{m}-\sqrt{n}}{\sqrt[4]{m}-\sqrt[4]{n}}=[x=\sqrt[4]{m},\ y=\sqrt[4]{n}]=
\cfrac{x^4-y^4}{x^2(x-y)}-\cfrac{x^2-y^2}{x-y}=\cfrac{x^4-y^4}{x^2(x-y)}-\cfrac{x^2-y^2}{x-y}=\cfrac{x^4-y^4-x^4+x^2y^2}{x^2(x-y)}=
\cfrac{y^2(x-y)(x+y)}{x^2(x-y)}=\cfrac{y^2(x+y)}{x^2}=(\sqrt[4]{m}+\sqrt[4]{n})\sqrt{\cfrac{n}{m}}.$\\
25. $\left(\cfrac{x\sqrt{x}-8}{x-3\sqrt{x}+2}-\cfrac{6\sqrt{x}}{\sqrt{x}-1}
ight):
\left(1-\cfrac{1}{\sqrt{x}-1}
ight)=[a=\sqrt{x}]=
\left(\cfrac{a^3-8}{a^2-3a+2}-\cfrac{6a}{a-1}
ight):\left(1-\cfrac{1}{a-1}
ight)=
\left(\cfrac{(a-2)(a^2+2a+4)}{(a-2)(a-1)}-\cfrac{6a}{a-1}
ight):\left(\cfrac{a-2}{a-1}
ight)=
\cfrac{a^2+2a+4-6a}{a-1}\cdot\cfrac{a-1}{a-2}=\cfrac{(a-2)^2}{a-1}\cdot\cfrac{a-1}{a-2}=a-2=\sqrt{x}-2.$\\
26. $\left(\cfrac{x\sqrt{x}+1}{x-\sqrt{x}-2}+\cfrac{3\sqrt{x}}{\sqrt{x}-2}
ight):
\left(\cfrac{1}{3}+\cfrac{1}{\sqrt{x}-2}
ight)=[a=\sqrt{x}]=
\left(\cfrac{a^3+1}{a^2-a-2}+\cfrac{3a}{a-2}
ight):\left(\cfrac{1}{3}+\cfrac{1}{a-2}
ight)=
\left(\cfrac{(a+1)(a^2-a+1)}{(a+1)(a-2)}+\cfrac{3a}{a-2}
ight):\left(\cfrac{a-2+3}{3(a-2)}
ight)=
\cfrac{a^2-a+1+3a}{a-2}\cdot\cfrac{3(a-2)}{a+1}=\cfrac{(a+1)^2}{a-2}\cdot\cfrac{3(a-2)}{a+1}=3a+3=3(\sqrt{x}+1).$\\
27. $\left(\cfrac{\sqrt{x^3}+\sqrt{y^3}}{x-\sqrt{x}\sqrt{y}+y}+
2xy\cfrac{(\sqrt{x})^{-1}-(\sqrt{y})^{-1}}{x-y}
ight)(\sqrt{x}+\sqrt{y})=[a=\sqrt{x},\ b=\sqrt{y}]=$\\$
\left(\cfrac{a^3+b^3}{a^2-ab+b^2}+2a^2b^2\cfrac{\cfrac{1}{a}-\cfrac{1}{b}}{a^2-b^2}
ight)(a+b)=
\left(a+b+2a^2b^2\cfrac{b-a}{ba(a-b)(a+b)}
ight)(a+b)=\left(a+b-\cfrac{2ab}{a+b}
ight)(a+b)=
\cfrac{a^2+2ab+b^2-2ab}{a+b}\cdot(a+b)=a^2+b^2=x+y.$\\
28. $\left(\cfrac{\sqrt{a^3}-\sqrt{b^3}}{a+\sqrt{a}\sqrt{b}+b}+
2ab\cfrac{(\sqrt{a})^{-1}+(\sqrt{b})^{-1}}{a-b}
ight)(\sqrt{a}-\sqrt{b})=[x=\sqrt{a},\ y=\sqrt{b}]=$\\$
\left(\cfrac{x^3-y^3}{x^2+xy+y^2}+2x^2y^2\cfrac{\cfrac{1}{x}+\cfrac{1}{y}}{x^2-y^2}
ight)(x-y)=
\left(x-y+2x^2y^2\cfrac{x+y}{xy(x-y)(x+y)}
ight)(x-y)=$\\$\left(x-y+\cfrac{2xy}{x-y}
ight)(x-y)=
\cfrac{x^2-2xy+y^2+2xy}{x-y}\cdot(x-y)=x^2+y^2=a+b.$\\
29. $\cfrac{3\cdot\sqrt{x^2y}-x\sqrt{25y}}{\sqrt{64x^4y^3}}=\cfrac{-3x\sqrt{y}-5x\sqrt{y}}{8x^2y\sqrt{y}}=\cfrac{-8x\sqrt{y}}{8x^2y\sqrt{y}}=-\cfrac{1}{xy}.$\\
30. $\cfrac{4\cdot\sqrt{x^2y}+x\sqrt{9y}}{\sqrt{x^4y^3}}=\cfrac{-4x\sqrt{y}+3x\sqrt{y}}{x^2y\sqrt{y}}=\cfrac{-x\sqrt{y}}{x^2y\sqrt{y}}=-\cfrac{1}{xy}.$\\
31. $\cfrac{a^2+8a+15}{\sqrt{a^2+10a+25}}+\cfrac{a^2+3a+2}{\sqrt{a^2+2a+1}}=\cfrac{(a+3)(a+5)}{\sqrt{(a+5)^2}}+\cfrac{(a+2)(a+1)}{\sqrt{(a+1)^2}}=
\cfrac{(a+3)(a+5)}{a+5}+\cfrac{(a+2)(a+1)}{-(a+1)}=a+3-a-2=1.$\\
32. $\cfrac{a^2+9a+20}{\sqrt{a^2+8a+16}}+\cfrac{a^2+8a+12}{\sqrt{a^2+4a+4}}=\cfrac{(a+4)(a+5)}{\sqrt{(a+4)^2}}+\cfrac{(a+6)(a+2)}{\sqrt{(a+2)^2}}=
\cfrac{(a+4)(a+5)}{a+4}+\cfrac{(a+6)(a+2)}{-(a+2)}=a+5-a-6=-1.$\\
33. $\left(\cfrac{1}{(a^\frac{1}{2}+b^\frac{1}{2})^{-2}}-\cfrac{a^\frac{3}{2}+
b^\frac{3}{2}}{a^\frac{1}{2}+
b^\frac{1}{2}}
ight)^2\cdot\left(\cfrac{27a^{-3}}{64b^{-6}}
ight)^{-\frac{1}{3}}=[x=a^\frac{1}{2},\ y=b^\frac{1}{2}]=
\left(\cfrac{1}{(x+y)^{-2}}-\cfrac{x^3+y^3}{x+y}
ight)^2\cdot\cfrac{3a}{4b^2}=$\\$
\left(x^2+2xy+y^2-x^2+xy-y^2
ight)^2\cdot\cfrac{4a}{3b^2}=
9x^2y^2\cdot\cfrac{4a}{3b^2}=9ab\cfrac{4a}{3b^2}=\cfrac{12a^2}{b}.$\\
34. $\left(\cfrac{d^3-8}{d^2-4}-\cfrac{6d}{d+2}
ight):\left(1-\cfrac{4}{d+2}
ight)^2=
\left(\cfrac{(d-2)(d^2+2d+4)}{(d-2)(d+2)}-\cfrac{6d}{d+2}
ight):\left(\cfrac{d+2-4}{d+2}
ight)^2=$\\$
\cfrac{d^2+2d+4-6d}{d+2}\cdot\cfrac{(d+2)^2}{(d-2)^2}=\cfrac{(d-2)^2}{d+2}\cdot\cfrac{(d+2)^2}{(d-2)^2}=d+2.$\\
35. $\cfrac{x+40}{x^3-16x}:\left(\cfrac{x-4}{3x^2+11x-4}-\cfrac{16}{16-x^2}
ight)=
\cfrac{x+40}{x(x-4)(x+4)}:\left(\cfrac{x-4}{(3x-1)(x+4)}+\cfrac{16}{(x-4)(x+4)}
ight)=
\cfrac{x+40}{x(x-4)(x+4)}:\cfrac{x^2-8x+16+48x-16}{(3x-1)(x-4)(x+4)}=
\cfrac{x+40}{x(x-4)(x+4)}\cdot\cfrac{(3x-1)(x-4)(x+4)}{x(x+40)}=\cfrac{3x-1}{x^2}.$\\
36. $\left(\left(x^\frac{5}{6}-\sqrt[3]{x}
ight):\left(\left(
\cfrac{x^\frac{3}{4}-1}{x^\frac{1}{4}-1}-x^\frac{1}{2}
ight)\cdot
\left(
\cfrac{x^\frac{3}{4}+1}{x^\frac{1}{4}+1}-x^\frac{1}{2}
ight)
ight)
ight)^{-3}=[a=x^\frac{1}{12}]=$\\$
\left(\left(a^{10}-a^4
ight):\left(\left(\cfrac{a^9-1}{a^3-1}-a^6
ight)\cdot\left(\cfrac{a^9+1}{a^3+1}-a^6
ight)
ight)
ight)^{-3}=$\\$
\left(a^4(a^6-1):\left(\left(a^6+a^3+1-a^6
ight)\cdot\left(a^6-a^3+1-a^6
ight)
ight)
ight)^{-3}=
\left(a^4(a^6-1):\left(\left(a^3+1
ight)\cdot\left(1-a^3
ight)
ight)
ight)^{-3}=$\\$
\left(a^4(a^6-1):\left(1-a^6
ight)
ight)^{-3}=(-a^4)^{-3}=-\cfrac{1}{a^{12}}=-\cfrac{1}{x}.$\\
37. $\cfrac{(x^2-y^2)(\sqrt[3]{x}+\sqrt[3]{y})}{\sqrt[3]{x^5}+\sqrt[3]{x^2y^3}-
\sqrt[3]{x^3y^2}-\sqrt[3]{y^5}}-\cfrac{x\sqrt[3]{y}+\sqrt[3]{y^4}}{(\sqrt[3]{x}-
\sqrt[3]{y})^2+\sqrt[3]{xy}}=[a=\sqrt[3]{x},\ b=\sqrt[3]{y}]=
\cfrac{(a^6-b^6)(a+b)}{a^5+a^2b^3-a^3b^2-b^5}-\cfrac{a^3b+b^4}{(a-b)^2+ab}=
\cfrac{(a^6-b^6)(a+b)}{a^2(a^3+b^3)-b^2(a^3+b^3)}-\cfrac{b(a^3+b^3)}{a^2-2ab+b^2+ab}=
\cfrac{(a-b)(a^2+ab+b^2)(a^3+b^3)(a+b)}{(a^3+b^3)(a-b)(a+b)}-\cfrac{b(a+b)(a^2-ab+b^2)}{a^2-ab+b^2}=
a^2+ab+b^2-ab-b^2=a^2=\sqrt[3]{x^2}.$\\
38. $\cfrac{x^3+5x^2+3x-9}{x-1}=\cfrac{x^3-1+5(x^2-1)+3(x-1)}{x-1}=$\\$\cfrac{(x-1)(x^2+x+1)+5(x-1)(x+1)+3(x-1)}{x-1}=
\cfrac{(x-1)(x^2+x+1)+5(x-1)(x+1)+3(x-1)}{x-1}=$\\$\cfrac{(x-1)(x^2+x+1+5x+5+3)}{x-1}=x^2+6x+9=(x+3)^2.$\\
39. $\cfrac{x^3-5x^2+3x+9}{x+1}=\cfrac{x^3+1-5(x^2-1)+3(x+1)}{x+1}=$\\$\cfrac{(x+1)(x^2-x+1)-5(x+1)(x-1)+3(x+1)}{x+1}=
\cfrac{(x+1)(x^2-x+1-5x+5+3)}{x+1}=x^2-6x+9=(x-3)^2.$\\
40. $\left(\sqrt{a}+\cfrac{b}{\sqrt{a}-\sqrt{b}}
ight)\left(1-\cfrac{\sqrt{b^3}}{a\sqrt{a}+b\sqrt{b}}
ight)
(\sqrt{a}+\sqrt{b})=[x=\sqrt{a},\ y=\sqrt{b}]=\left(x+\cfrac{y^2}{x-y}
ight)\left(1-\cfrac{x^3}{x^3+y^3}
ight)$\\$(x+y)=
\cfrac{x^2-xy+y^2}{x-y}\cdot\cfrac{x^3+y^3-x^3}{(x+y)(x^2-xy+y^2}(x+y)=\cfrac{y^3}{x-y}=\cfrac{a\sqrt{a}}{\sqrt{a}-\sqrt{b}}.$\\
41. $\left(\sqrt{a}+\cfrac{b}{\sqrt{a}+\sqrt{b}}
ight)\left(1+\cfrac{\sqrt{b^3}}{a\sqrt{a}-b\sqrt{b}}
ight)
(\sqrt{a}-\sqrt{b})=[x=\sqrt{a},\ y=\sqrt{b}]=\left(x+\cfrac{y^2}{x+y}
ight)\left(1+\cfrac{y^3}{x^3-y^3}
ight)$\\$
(x-y)=\cfrac{x^2+xy+y^2}{x+y}\cdot\cfrac{x^3-y^3+y^3}{(x-y)(x^2+xy+y^2)}(x-y)=\cfrac{x^3}{x+y}=\cfrac{a\sqrt{a}}{\sqrt{a}+\sqrt{b}}.$\\
42. $\left(\cfrac{a\sqrt{a}+b\sqrt{b}}{\sqrt{a}+\sqrt{b}}-\sqrt{ab}
ight):(a-b)+\cfrac{2\sqrt{b}}{\sqrt{a}+\sqrt{b}}=[x=\sqrt{a},\ y=\sqrt{b}]=
\left(\cfrac{x^3+y^3}{x+y}-xy
ight):(x^2-y^2)+\cfrac{2y}{x+y}=
\left(x^2-xy+y^2-xy
ight):((x-y)(x+y))+\cfrac{2y}{x+y}=(x-y)^2:((x-y)(x+y))+\cfrac{2y}{x+y}=\cfrac{x-y+2y}{x+y}=1.$\\
43. $\left(\cfrac{2}{\sqrt{a}-\sqrt{b}}-\cfrac{2\sqrt{a}}{a\sqrt{a}+b\sqrt{b}}\cdot\cfrac{a-\sqrt{ab}+b}{\sqrt{a}-\sqrt{b}}
ight):4\sqrt{b}=[x=\sqrt{a},\ y=\sqrt{b}]=$\\$\left(\cfrac{2}{x-y}-\cfrac{2x}{x^3+y^3}\cdot\cfrac{x^2-xy+y^2}{x-y}
ight):4y=
\left(\cfrac{2}{x-y}-\cfrac{2x}{(x+y)(x^2-xy+y^2)}\cdot\cfrac{x^2-xy+y^2}{x-y}
ight):4y=$\\$
\left(\cfrac{2}{x-y}-\cfrac{2x}{(x+y)(x-y)}
ight):4y=
\cfrac{2x+2y-2x}{(x+y)(x-y)}:4y=\cfrac{1}{2(x^2-y^2)}=\cfrac{1}{2(a-b)}.$\\
44. $\cfrac{x-y}{\sqrt{x}-\sqrt{y}}:\left(\left(x^\frac{1}{4}-y^\frac{1}{4}
ight)^{-1}+\left(x^\frac{1}{4}+y^\frac{1}{4}
ight)^{-1}
ight)^{-2}=[a=x^{\frac{1}{4}},\ b=y^\frac{1}{4}]=\cfrac{a^4-b^4}{a^2-b^2}:\left(\cfrac{1}{a-b}+\cfrac{1}{a+b}
ight)^{-2}=
(a^2+b^2)\cdot\left(\cfrac{a+b+a-b}{a^2-b^2}
ight)^{2}=(a^2+b^2)\cfrac{4a^2}{(a^2-b^2)^2}=\cfrac{4a^2(a^2+b^2)}{(a^2-b^2)^2}=\cfrac{4\sqrt{x}(\sqrt{x}+\sqrt{y})}{(\sqrt{x}-\sqrt{y})^2}.$\\
45. $\cfrac{a+8b}{a^\frac{2}{3}-4b^\frac{2}{3}}:\cfrac{a^\frac{2}{3}b^\frac{1}{3}-2a^\frac{1}{3}b^\frac{2}{3}+4b}{a^\frac{2}{3}-2b^\frac{1}{3}a^\frac{1}{3}}=
[x=a^\frac{1}{3},\ y=b^\frac{b}{3}]=\cfrac{x^3+8y^3}{x^2-4y^2}:\cfrac{x^2y-2xy^2+4y^3}{x^2-2yx}=$\\$
\cfrac{(x+2y)(x^2-2xy+4y^2)}{(x-2y)(x+2y)}\cdot\cfrac{x(x-2y)}{y(x^2-2xy+4y^2)}=\cfrac{x}{y}=\left(\cfrac{a}{b}
ight)^\frac{1}{3}.$\\
46. $\left(\cfrac{a^{\frac{3}{2}}+b^{\frac{3}{2}}}{a^{\frac{1}{2}}+b^{\frac{1}{2}}}-(a+b)
ight)\cdot\cfrac{b^{\frac{1}{2}}-a^{\frac{1}{2}}}{a^{\frac{1}{2}}b^{\frac{3}{2}}-b^{\frac{1}{2}}a^{\frac{3}{2}}}=
[x=a^{\frac{1}{2}}, y=b^{\frac{1}{2}}]=
\left(\cfrac{x^3+y^3}{x+y}-(x^2+y^2)
ight)\cdot\cfrac{y-x}{xy^3-yx^3}=$\\$\left(\cfrac{(x+y)(x^2-xy+y^2)}{x+y}-x^2-y^2
ight)\cdot\cfrac{y-x}{xy(y-x)(y+x)}=
\left(x^2-xy+y^2-x^2-y^2
ight)\cdot\cfrac{1}{xy(y+x)}=$\\$-xy\cdot\cfrac{1}{xy(y+x)}=-\cfrac{1}{x+y}=-\cfrac{1}{a^{\frac{1}{2}}+b^{\frac{1}{2}}}=\cfrac{\sqrt{b}-\sqrt{a}}{a-b}.$\\
47. $\left(\cfrac{a^{\frac{3}{2}}-b^{\frac{3}{2}}}{a^{\frac{1}{2}}-b^{\frac{1}{2}}}-(a^{\frac{1}{2}}b^{\frac{1}{2}}+2b)
ight):\cfrac{ab^{\frac{1}{2}}-ba^{\frac{1}{2}}}{a^{\frac{1}{2}}b^{\frac{1}{2}}}=
[x=a^{\frac{1}{2}}, y=b^{\frac{1}{2}}]=
\left(\cfrac{x^3-y^3}{x-y}-(xy+2y^2)
ight):\cfrac{x^2y-y^2x}{xy}=$\\$\left(\cfrac{(x-y)(x^2+xy+y^2)}{x-y}-xy-2y^2
ight)\cdot\cfrac{xy}{xy(x-y)}=
(x^2+xy+y^2-xy-2y^2)\cdot\cfrac{1}{x-y}=(x-y)(x+y)\cdot\cfrac{1}{x-y}=x+y=\sqrt{a}+\sqrt{b}.$\\
48.$x\left(\left(\cfrac{x^6-8}{x^4+2x^2+4}
ight)^{-1}-(x^2+2)^{-1}
ight)+(4-x^4)^{-1}:x^{-5}=
x\left(\left(\cfrac{(x^2-2)(x^4+2x^2+4)}{x^4+2x^2+4}
ight)^{-1}-\cfrac{1}{x^2+2}
ight)+\cfrac{x^5}{(2-x^2)(2+x^2)}=
x\left(\cfrac{1}{x^2-2}-\cfrac{1}{x^2+2}
ight)-\cfrac{x^5}{(x^2-2)(x^2+2)}=
x\cdot\cfrac{x^2+2-x^2+2}{(x^2-2)(x^2+2)}-\cfrac{x^5}{(x^2-2)(x^2+2)}=\cfrac{4x-x^5}{(x^2-2)(x^2+2)}=
\cfrac{x(2-x^2)(2+x^2)}{(x^2-2)(x^2+2)}=-x.$\\
49. $(x^3-3x)^{-1}-\left(\cfrac{x^7+27x}{x^4-3x^2+9}
ight)^{-1}-2x^3\cdot(3x^4-27)^{-1}=
\cfrac{1}{x(x^2-3)}-\left(\cfrac{x(x^2+3)(x^4-3x^2+9)}{x^4-3x^2+9}
ight)^{-1}-\cfrac{2x^3}{3(x^2-3)(x^2+3)}=
\cfrac{1}{x(x^2-3)}-\cfrac{1}{x(x^2+3)}-\cfrac{2x^3}{3(x^2-3)(x^2+3)}=
\cfrac{x^2+3-x^2+3}{x(x^2-3)(x^2+3)}-\cfrac{2x^3}{3(x^2-3)(x^2+3)}=
\cfrac{18-2x^4}{3x(x^2-3)(x^2+3)}=\cfrac{2(3-x^2)(3+x^2)}{3x(x^2-3)(x^2+3)}=-\cfrac{2}{3x}.$\\
50. $4ab+\cfrac{\left(1+\left(\cfrac{a}{b}
ight)^{-3}
ight)a^3}{(\sqrt{a}+\sqrt{b})^2-2\sqrt{ab}}-\cfrac{\left(\cfrac{\sqrt{a}+\sqrt{b}}{2b\sqrt{a}}
ight)^{-1}+
\left(\cfrac{\sqrt{a}+\sqrt{b}}{2a\sqrt{b}}
ight)^{-1}}{\left(\cfrac{a+\sqrt{ab}}{2}
ight)^{-1}+\left(\cfrac{b+\sqrt{ab}}{2}
ight)^{-1}}=$\\$
4ab+\cfrac{\left(1+\cfrac{b^3}{a^3}
ight)a^3}{a+2\sqrt{ab}+b-2\sqrt{ab}}-\cfrac{\cfrac{2b\sqrt{a}}{\sqrt{a}+\sqrt{b}}+
\cfrac{2a\sqrt{b}}{\sqrt{a}+\sqrt{b}}}{\cfrac{2}{a+\sqrt{ab}}+\cfrac{2}{b+\sqrt{ab}}}=
4ab+\cfrac{a^3+b^3}{a+b}-\cfrac{\cfrac{2\sqrt{a}\sqrt{b}(\sqrt{a}+\sqrt{b})}{\sqrt{a}+\sqrt{b}}}{\cfrac{2}{\sqrt{a}(\sqrt{a}+\sqrt{b})}+\cfrac{2}{\sqrt{b}(\sqrt{a}+\sqrt{b})}}=
4ab+a^2-ab+b^2-\cfrac{2\sqrt{ab}}{\cfrac{2(\sqrt{a}+\sqrt{b})}{\sqrt{ab}(\sqrt{a}+\sqrt{b})}}=
a^2+3ab+b^2-\cfrac{2\sqrt{ab}}{\cfrac{2}{\sqrt{ab}}}=a^2+3ab+b^2-ab=(a+b)^2.$\\
51. $\cfrac{x^\frac{1}{2}+1}{x^\frac{3}{2}+x+x^\frac{1}{2}}:\cfrac{1}{x^2-x^\frac{1}{2}}=
[a=x^\frac{1}{2}]=\cfrac{a+1}{a^3+a^2+a}:\cfrac{1}{a^4-a}=
\cfrac{a+1}{a(a^2+a+1)}\cdot a(a-1)(a^2+a+1)=a^2-1=x-1.$\\
52. $\cfrac{a^2+a^\frac{1}{2}}{a^\frac{1}{2}+1}\cdot\cfrac{a^\frac{1}{2}-1}{a^\frac{3}{2}-a+a^\frac{1}{2}}=
[x=a^\frac{1}{2}]=\cfrac{x^4+x}{x+1}\cdot\cfrac{x-1}{x^3-x^2+x}
=\cfrac{x(x+1)(x^2-x+1)}{x+1}\cdot\cfrac{x-1}{x(x^2-x+1)}=
x-1=\sqrt{a}-1.$\\
53. $\cfrac{2ab(a^3-b^3)}{a^2+ab+b^2}-\cfrac{(a-b)(a^4-b^4)}{a^2-b^2}=
\cfrac{2ab(a-b)(a^2+ab+b^2)}{a^2+ab+b^2}-\cfrac{(a-b)(a^2-b^2)(a^2+b^2)}{a^2-b^2}=
2ab(a-b)-(a-b)(a^2+b^2)=(b-a)(a^2-2ab+b^2)=(b-a)^3=7^3=343.$

ewpage
