1. $\left(\left(\cfrac{\sqrt{a}+\sqrt{b}}{\sqrt[4]{a}-\sqrt[4]{b}}
ight)^{-1}-
\cfrac{2\sqrt[4]{ab}}{b^{\frac{3}{4}}-a^{\frac{1}{4}}b^{\frac{1}{2}}+
a^{\frac{1}{2}}b^{\frac{1}{4}}-a^{\frac{3}{4}}}
ight)^{-1}=[x=\sqrt[4]{a},\ y=\sqrt[4]{b}]=$\\$
\left(\cfrac{x-y}{x^2+y^2}-\cfrac{2xy}{y^3-xy^2+x^2y-x^3}
ight)^{-1}=
\left(\cfrac{x-y}{x^2+y^2}-\cfrac{2xy}{y^2(y-x)+x^2(y-x)}
ight)^{-1}=$\\$
\left(\cfrac{x-y}{x^2+y^2}-\cfrac{2xy}{(y-x)(x^2+y^2)}
ight)^{-1}=
\left(\cfrac{x-y}{x^2+y^2}+\cfrac{2xy}{(x-y)(x^2+y^2)}
ight)^{-1}=
\left(\cfrac{x^2-2xy+y^2+2xy}{(x-y)(x^2+y^2)}
ight)^{-1}=$\\$x-y=\sqrt[4]{a}-\sqrt[4]{b}.$\\
