36. $\left(\left(x^\frac{5}{6}-\sqrt[3]{x}
ight):\left(\left(
\cfrac{x^\frac{3}{4}-1}{x^\frac{1}{4}-1}-x^\frac{1}{2}
ight)\cdot
\left(
\cfrac{x^\frac{3}{4}+1}{x^\frac{1}{4}+1}-x^\frac{1}{2}
ight)
ight)
ight)^{-3}=[a=x^\frac{1}{12}]=$\\$
\left(\left(a^{10}-a^4
ight):\left(\left(\cfrac{a^9-1}{a^3-1}-a^6
ight)\cdot\left(\cfrac{a^9+1}{a^3+1}-a^6
ight)
ight)
ight)^{-3}=$\\$
\left(a^4(a^6-1):\left(\left(a^6+a^3+1-a^6
ight)\cdot\left(a^6-a^3+1-a^6
ight)
ight)
ight)^{-3}=
\left(a^4(a^6-1):\left(\left(a^3+1
ight)\cdot\left(1-a^3
ight)
ight)
ight)^{-3}=$\\$
\left(a^4(a^6-1):\left(1-a^6
ight)
ight)^{-3}=(-a^4)^{-3}=-\cfrac{1}{a^{12}}=-\cfrac{1}{x}.$\\
