37. $\cfrac{(x^2-y^2)(\sqrt[3]{x}+\sqrt[3]{y})}{\sqrt[3]{x^5}+\sqrt[3]{x^2y^3}-
\sqrt[3]{x^3y^2}-\sqrt[3]{y^5}}-\cfrac{x\sqrt[3]{y}+\sqrt[3]{y^4}}{(\sqrt[3]{x}-
\sqrt[3]{y})^2+\sqrt[3]{xy}}=[a=\sqrt[3]{x},\ b=\sqrt[3]{y}]=
\cfrac{(a^6-b^6)(a+b)}{a^5+a^2b^3-a^3b^2-b^5}-\cfrac{a^3b+b^4}{(a-b)^2+ab}=
\cfrac{(a^6-b^6)(a+b)}{a^2(a^3+b^3)-b^2(a^3+b^3)}-\cfrac{b(a^3+b^3)}{a^2-2ab+b^2+ab}=
\cfrac{(a-b)(a^2+ab+b^2)(a^3+b^3)(a+b)}{(a^3+b^3)(a-b)(a+b)}-\cfrac{b(a+b)(a^2-ab+b^2)}{a^2-ab+b^2}=
a^2+ab+b^2-ab-b^2=a^2=\sqrt[3]{x^2}.$\\
