70. $\left(1-\cfrac{3}{2-a}
ight)^2=\left(\cfrac{2-a-3}{2-a}
ight)^2=\left(\cfrac{-1-a}{2-a}
ight)^2=\cfrac{(a+1)^2}{(a-2)^2}.$\\
$\cfrac{2a+1}{a^2-6a+5}-\cfrac{11}{4a-20}=\cfrac{2a+1}{a(a-5)-(a-5)}-\cfrac{11}{4(a-5)}=\cfrac{2a+1}{(a-5)(a-1)}-\cfrac{11}{4(a-5)}=
\cfrac{8a+4-11a+11}{4(a-5)(a-1)}=$\\$=\cfrac{-3(a-5)}{4(a-5)(a-1)}=\cfrac{-3}{4(a-1)}.$\\
$\cfrac{-3}{4(a-1)}:\cfrac{a^2-4a+4}{4a^2-4}=\cfrac{-3}{4(a-1)}\cdot\cfrac{4(a-1)(a+1)}{(a-2)^2}=\cfrac{-3(a+1)}{(a-2)^2}.$\\
$\cfrac{(a+1)^2}{(a-2)^2}+\cfrac{-3(a+1)}{(a-2)^2}=\cfrac{(a+1)(a+1-3)}{(a-2)^2}=\cfrac{(a+1)(a-2)}{(a-2)^2}=\cfrac{a+1}{a-2}.$\\
