148. $\cfrac{4}{a+2}+\cfrac{4a^2+10a}{4a+9}\cdot\left(\cfrac{4a+1}{2a^2+a-10}-\cfrac{4}{a^2-4}
ight)-1=
\cfrac{4}{a+2}+\cfrac{2a(2a+5)}{4a+9}\cdot\Big(\cfrac{4a+1}{2(a^2-4)+a-2}-$\\$\cfrac{4}{(a-2)(a+2)}\Big)-1=
\cfrac{4}{a+2}+\cfrac{2a(2a+5)}{4a+9}\cdot\left(\cfrac{4a+1}{(a-2)(2a+5)}-\cfrac{4}{(a-2)(a+2)}
ight)-1=
\cfrac{4}{a+2}+\cfrac{2a(2a+5)}{4a+9}\cdot\cfrac{(4a+1)(a+2)-4(2a+5)}{(a-2)(a+2)(2a+5)}-1=
\cfrac{4}{a+2}+\cfrac{2a}{4a+9}\cdot\cfrac{4a^2+a-18}{(a-2)(a+2)}-1=
\cfrac{4}{a+2}+\cfrac{2a}{4a+9}\cdot\cfrac{4(a^2-4)+a-2}{(a-2)(a+2)}-1=
\cfrac{4}{a+2}+\cfrac{2a}{4a+9}\cdot\cfrac{(a-2)(4a+9)}{(a-2)(a+2)}-1=
\cfrac{4}{a+2}+\cfrac{2a}{a+2}-1=1.$

ewpage
