71. $\left(1-\cfrac{5}{3-b}
ight)^2=\left(\cfrac{3-b-5}{3-b}
ight)^2=\left(\cfrac{-2-b}{3-b}
ight)^2=\cfrac{(b+2)^2}{(b-3)^2}.$\\
$\cfrac{2b+1}{b^2-6b+8}-\cfrac{9}{2b-8}=\cfrac{2b+1}{b(b-2)-4(b-2)}-\cfrac{9}{2(b-4)}=\cfrac{2b+1}{(b-2)(b-4)}-\cfrac{9}{2(b-4)}=
\cfrac{4b+2-9b+18}{2(b-2)(b-4)}=$\\$=\cfrac{-5(b-4)}{2(b-2)(b-4)}=\cfrac{-5}{2(b-2)}.$\\
$\cfrac{-5}{2(b-2)}:\cfrac{b^2-6b+9}{2b^2-8}=\cfrac{-5}{2(b-2)}\cdot\cfrac{2(b-2)(b+2)}{(b-3)^2}=\cfrac{-5(b+2)}{(b-3)^2}.$\\
$\cfrac{(b+2)^2}{(b-3)^2}+\cfrac{-5(b+2)}{(b-3)^2}=\cfrac{(b+2)(b+2-5)}{(b-3)^2}=\cfrac{(b+2)(b-3)}{(b-3)^2}=\cfrac{b+2}{b-3}.$\\
