3. $\cfrac{\cfrac{1}{c}+\cfrac{1}{a+b}}{\cfrac{1}{c}-\cfrac{1}{a-b}}=
\cfrac{\cfrac{a+b}{(a+b)c}+\cfrac{c}{(a+b)c}}{\cfrac{a-b}{(a-b)c}-\cfrac{c}{(a-b)c}}=
\cfrac{\cfrac{a+b+c}{(a+b)c}}{\cfrac{a-b-c}{(a-b)c}}=\cfrac{a+b+c}{(a+b)c}\cdot\cfrac{(a-b)c}{a-b-c}=\cfrac{(a+b+c)(a-b)}{(a-b-c)(a+b)}.$\\
$\cfrac{c^2+2bc}{a^2-b^2}-1=\cfrac{c^2+2bc-a^2+b^2}{a^2-b^2}=\cfrac{(b+c)^2-a^2}{(a-b)(a+b)}=\cfrac{(b+c-a)(b+c+a)}{(a-b)(a+b)}.$\\
$\left(1+\cfrac{c}{a+b}
ight)^2=\left(\cfrac{a+b+c}{a+b}
ight)^2=\cfrac{(a+b+c)^2}{(a+b)^2}.$\\
$\cfrac{(a+b+c)(a-b)}{(a-b-c)(a+b)}\cdot\cfrac{(b+c-a)(b+c+a)}{(a-b)(a+b)}:\cfrac{(a+b+c)^2}{(a+b)^2}=$\\$=
\cfrac{(a+b+c)(a-b)}{(a-b-c)(a+b)}\cdot\cfrac{(b+c-a)(b+c+a)}{(a-b)(a+b)}\cdot\cfrac{(a+b)^2}{(a+b+c)^2}=-1.$\\
