\section{Уравнения задачи}
$\begin{array}{ll}
1.\ \cfrac{x+1}{2x-3}+\cfrac{x}{x+1}=\cfrac{x^2+6x-5}{2x^2-x-3},&
2.\ \cfrac{x+2}{2x-1}+\cfrac{x+1}{x+2}=\cfrac{x^2+8x+2}{2x^2+3x-2},\\
3.\ \sqrt{x-2}\cdot\sqrt{x-8}=4,&
4.\ \sqrt{x-1}\cdot\sqrt{x-4}=2,\\
5.\ ||3+x|+2|=2x,&
6.\ ||2+x|+3|=3x,\\
7.\ \cfrac{z^2-z}{z^2-z+1}-\cfrac{z^2-z+2}{z^2-z-2}=1,&
8.\ \cfrac{x^2+2x+1}{x^2+2x+2}+\cfrac{x^2+2x+2}{x^2+2x+3}=\cfrac{7}{6},\\
9.\ \sqrt{x^2+8x-4}=\sqrt{4x-4},&
10.\ \sqrt{x^2+9x-3}=\sqrt{3x-3},\\
11.\ |x-5|+|x-2|-|x+1|=-3,&
12.\ |x-7|-|x|=2-|x+1|,\\
13.\ \cfrac{1}{x+2}-\cfrac{1}{x+4}=\cfrac{1}{x+3}-\cfrac{1}{x+1},&
14.\ \cfrac{3}{x-2}-\cfrac{4}{x-1}=\cfrac{1}{x-4}-\cfrac{2}{x-3},\\
15.\ (x+2)\sqrt{x^2-x-20}=6x+12,&
16.\ (x-1)\sqrt{x^2-x-6}=6x-6,\\
17.\ |7x-12|-|11-7x|=1,&
18.\ |16-9x|-|9x-5|=11,\\
19.\ min(2x^2-x-4; x^2+3x+1)=3x+12,&
20.\ max(x^2+x-5;-2x^2+7x+4)=x-1,\\
21.\ \cfrac{2}{x^2-x+1}=\cfrac{1}{x+1}+\cfrac{2x-1}{x^3+1},&
22.\ \cfrac{2}{x+2}+\cfrac{1}{2}=-\cfrac{4}{x^2+2x},\\
23.\ |2x^2-x+1|=x-1,&
24.\ |2x^2-x+2|=x-2,\\
25.\ \sqrt{3x^2-6x+16}=2x-1,&
26.\ \sqrt{3x^2-11x+21}=2x-3,\\
27.\ \cfrac{2x+1}{1+x}=\cfrac{2}{x^2-1},&
28.\ \cfrac{1-2x}{x-1}=-\cfrac{2}{x^2-1},\\
29.\ x^2+2x+\sqrt{x^2+2x+8}=12,&
30.\ x^2-2x+\sqrt{x^2-2x+8}=12,\\
31.\ ||x-2|-1|=x,&
32.\ ||x+2|-1|=-x,\\
33.\ \begin{cases} x^2+3xy=1,\\ y-x=1.\end{cases},&
34.\ \begin{cases} x^2+3xy=1,\\ x-y=1.\end{cases},\\
35.\ \cfrac{44}{4-x^2}+\cfrac{2x+7}{x-2}=\cfrac{3-x}{x+2},&
36.\ \cfrac{x}{x+1}-\cfrac{9x+13}{x^2-2x-3}=\cfrac{5}{3-x},\\
37.\ (x+1)\sqrt{1+4x-x^2}=x^2-1,&
38.\ (x^2-8x)\sqrt{7-x}=x(x^2-9x+8),\\
39.\ \cfrac{1}{x^2+2x+4}+\cfrac{1}{x-2}=\cfrac{x^2-2x+4}{x^3-8},&
40.\ \cfrac{x^2+3x+9}{x^3+27}-\cfrac{1}{x+3}=\cfrac{2}{x^2-3x+9},\\
41.\ (x^2+3x+1)(x^2+3x+3)+1=0,&
42.\ (x^2-5x+2)(x^2-5x-1)=28,\\
43.\ x-3+4\sqrt{x-3}=12,&
44.\ x+2-13\sqrt{x+2}=-42,\\
45.\ \cfrac{11x-x^2-8}{2x^2-x-3}=\cfrac{x+1}{2x-3}+\cfrac{x}{x+1},&
46.\ \cfrac{9x-x^2+2}{2x^2+3x-2}=\cfrac{x+2}{2x-1}+\cfrac{x+1}{x+2},\end{array}$\\$\begin{array}{ll}
47.\ (x-1)^2+3|x-1|-4=0,&
48.\ (x-2)^2+|x-2|-6=0,\\
49.\ \cfrac{x}{\sqrt{1-x^2}}-2\cfrac{\sqrt{1-x^2}}{x}=-1,&
50.\ \cfrac{x-1}{\sqrt{x}}-2\cfrac{\sqrt{x}}{x-1}=1,\\
51.\ \sqrt{7-x}=x-1,&
52.\ x-\sqrt{x+1}=5,\\
53.\ |x+3|-|x-5|+|2x-5|=6,&
54.\ |x-2|-|x+4|+|2x-3|=1,\\
55.\ \cfrac{6}{(x+1)(x+2)}+\cfrac{8}{(x-1)(x+4)}=1,&
56.\ \cfrac{16}{(x+6)(x-1)}-\cfrac{20}{(x+2)(x+3)}=1,\\
57.\ \cfrac{x-4}{\sqrt{x}}-\cfrac{\sqrt{x}}{x-4}=\cfrac{8}{3},&
58.\ \sqrt{12-\cfrac{2}{x}-\cfrac{4x+1}{x+4}}=\cfrac{2}{x}+\cfrac{4x+1}{4+x},\\
59.\ 2x^2+3x-17=2(2-\sqrt{7})^2+3(2-\sqrt{7})-17,&
60.\ \sqrt{2x-1}=x-2,\\
61.\ 4x^2-9x-11=4(\sqrt{2}+\sqrt{3})^2-9(\sqrt{2}+\sqrt{3})-11,&
62.\ \sqrt{1+4x}=x+1,\\
63.\ \begin{cases}x^2-y=\cfrac{3}{4},\\ y^2+x=0,75.\end{cases}&
64.\ \begin{cases} \cfrac{6}{x+y}+\cfrac{5}{x-y}=7,\\ \cfrac{3}{x+y}-\cfrac{2}{x-y}=-1.\end{cases}\\
65.\ \left(\cfrac{x^2-3x+2}{x}
ight)^2-x=\cfrac{2-x}{x},&
66.\ \left(\cfrac{x^2-4x+7}{x}
ight)^2-x=\cfrac{7+2x}{x},\\
67.\ \sqrt{x-1}=x-3,&
68.\ \sqrt{x+2}=x,\\
69.\ |3-x|+|2x-5|=6,&
70.\ |2-x|+|2x-3|=1,\\
71.\ \cfrac{2x}{x-1}+\cfrac{3}{x-2}=6,&
72.\ \cfrac{4}{x+1}+\cfrac{3x}{x-2}=-1,\\
73.\ \sqrt{2x+5}-\sqrt{2x}=1,&
74.\ 2\sqrt{x-3}+\sqrt{x+1}=2,\\
75.\ \cfrac{x^2+4}{x}+\cfrac{x}{x^2+3x+4}+\cfrac{11}{2}=0,&
76.\ \cfrac{4(x^2+1)}{x^2-10x+1}-\cfrac{5x}{x^2+1}+\cfrac{7}{2}=0,\\
77.\ (x+1)(x^2+5x+6)=x+2,&
78.\ (x+3)(x^2+3x+2)=x+1,\\
79.\ (x^2-x-6)\sqrt{3x-2}=0,&
80.\ (x^2-x-2)\sqrt{2x+1}=0,\\
81.\ \sqrt{12-x}=-x,&
82.\ \sqrt{x+2}=-x,\\
83.\ (3x-2)(x-1)=4(x-1)^2,&
84.\ (3x+2)(x+1)=2(x+1)^2,\\
85.\ \cfrac{5}{x^2+2x+4}=\cfrac{1}{x-2}-\cfrac{4x+4}{x^3-8},&
86.\ \cfrac{4}{x^2+3x+9}=\cfrac{1}{x-3}-\cfrac{6x+9}{x^3-27},\\
87.\ \cfrac{2x-7}{x^2-9x+14}-\cfrac{1}{x^2-3x+2}=\cfrac{1}{x-1},&
88.\ \cfrac{2x+7}{x^2+5x-6}+\cfrac{3}{x^2+9x+18}=\cfrac{1}{x+3},\\
89.\ \cfrac{1}{|x^2-5x+6|}=\cfrac{|x-1,5|}{x^2-5x+6},&
90.\ \cfrac{|2x-1|}{8-x-x^2}-\cfrac{4}{|x^2+x-8|}=0,\\
91.\ \sqrt{5x+1}=x-1,&
92.\ |3x+2|=|7x-4|,\\
93.\ |4x-7|=|2x+3|,&
94.\ x^2-x=14-\cfrac{24}{x^2-x},\\
95.\ x^2-5x=30-\cfrac{144}{x^2-5x},&
96.\ \cfrac{4}{|x^2+10x|}=\cfrac{1}{25}+\cfrac{2}{5x},\\
97.\ \cfrac{25}{|x^2+5x|}=1+\cfrac{5}{x},&
98.\ \cfrac{1}{\cfrac{1}{\cfrac{1}{\sqrt{5}-2k}+4}+4}+4=\sqrt{5}+2,\\
99.\ 4-\cfrac{1}{4-\cfrac{1}{4-\cfrac{1}{2k-\sqrt{3}}}}=2-\sqrt{3},&
100.\ \left(\cfrac{x-1}{x+1}
ight)^2+\left(\cfrac{x}{x+3}
ight)^2=\cfrac{2(x^2-x)}{x^2+4x+3},\end{array}$\\
$\begin{array}{ll}
101.\ \left(\cfrac{x+1}{x-1}
ight)^2+\left(\cfrac{x}{x+5}
ight)^2=\cfrac{2x^2+2x}{x^2+4x-5},&
102.\ \sqrt{x+1}+3\sqrt{3x+7}=17-x,\\
103.\ x^2+2x+2|x+1|=7,&
104.\ (345x^2+137x-208)\sqrt{3x-2}=0,\\
105.\ \cfrac{8x-4x^2}{1-x^2}=\cfrac{x^3-4x}{x+1},&
106.\ (x-4)\sqrt{x^2-x-6}=6x-24,\\
107.\ (x+6)\sqrt{x^2-x-20}=6x+36,&
108.\ (x^2-3x)^2-2(x^2-3x)=8,\\
109.\ (x^2+4x)^2-2(x^2+4x)=15,\\
110.\ 4x^2-9x-11=4(\sqrt{5}+\sqrt{3})^2-9(\sqrt{5}+\sqrt{3})-11,\\
111.\ 2x^2+3x-17=2(2-\sqrt{5})^2+3(2-\sqrt{5})-17,&
112.\ \sqrt{2x^2+x+6}+\sqrt{2x^2+x-9}=5,\\
113.\ \sqrt{x^2+3x+6}-\sqrt{x^2+3x-1}=1,&
114.\ 2\cdot\left(\cfrac{x-1}{x+2}
ight)^2-\left(\cfrac{x+1}{x-2}
ight)^2=\cfrac{x^2-1}{x^2-4},\\
115.\ x^3-6x^2+12x-1=0,&
116.\ \sqrt{7-x}=x-2,\\
117.\ \sqrt{x+4}=x+1,&
118.\ |x+3|-|5-x|+|2x-5|=6,\\
119.\ |2x-3|+|2-x|-|x+4|=1,&
120.\ \sqrt{5-x}=x-2,\\
121.\ (x^2+2x)^2-(x+1)^2=55,&
122.\ |x^2+15x-64|=-15x,\\
123.\ (\sqrt{x^2+1}-1)^2=3\sqrt{x^2+1}+7,\end{array}$\\
$\begin{array}{ll}
124.\ (x^2+x-2)\sqrt{x+1}=(x-1)(x^2+3x+2),&
125.\ (x^2-3x-4)\sqrt{x-2}=(x+1)(x^2-6x+8),\\
126.\ \left(x+\cfrac{1}{x}
ight)^2+3x=4-\cfrac{3}{x},&
127.\ \left(x+\cfrac{1}{x}
ight)^2-2x=3+\cfrac{2}{x},\\
128.\ (x^2-2x)^2-3x^2+6x=4,&
129.\ x^2+x^{10}=2x^{12},\\
130.\ (2x^2-x-4)^2+16x^2-8x=17,&
131.\ 2\cdot(x^2+2x-5)^2+3x^2+6x=69,\\
132.\ (x^2-9)\cdot\sqrt{10-3x-x^2}=x^3-9x,&
133.\ (3x^2-12)\cdot\sqrt{x^2-4x-5}=8x-2x^3,\\
134.\ \sqrt{3x-2}=2-x,&
135.\ \sqrt{5x+2x^2}-x=2,\\
136.\ \cfrac{2|x|-6}{|x|+3}=\cfrac{x^2-9}{|x|+7},&
137.\ \cfrac{4|x|-16}{|x|+4}=\cfrac{x^2-16}{|x|+7},\\
138.\ (x^2-1)^2+x^2=2x^3-2x,&
139.\ (x^2-3)^2+x^2=2x^3-6x,\\
140.\ \cfrac{x+1}{x-1}=\cfrac{x^2-4x+3}{x-3},&
141.\ \cfrac{x+4}{x-2}=\cfrac{x^2-7x+10}{x-5},\\
142.\ \cfrac{\sqrt{x}+1}{2\sqrt{x}-1}=\cfrac{x+3\sqrt{x}+2}{\sqrt{x}},&
143.\ \cfrac{2\sqrt{x}+1}{\sqrt{x}-1}=\cfrac{2x+3\sqrt{x}+1}{\sqrt{x}},
\end{array}$\\
144.$ (x^2+x-2)\left(\cfrac{x^3-8}{x-2}-2(\sqrt{x^2+2x-3})^2
+x-4
ight)=0.$\qquad
145. $\begin{cases} x^2+3y+z=-8,\\ x+y^2+5z=-12,\\ x+y+z^2=6.\end{cases}$

ewpage
