133. $(3x^2-12)\cdot\sqrt{x^2-4x-5}=8x-2x^3\Leftrightarrow 3(x-2)(x+2)\cdot\sqrt{x^2-4x-5}=2x(2-x)(2+x).$ Из возможных корней $x=-2$ и $x=2$ подходит только $x=-2,$ так как при $x=2$ под корнем оказывается отрицательное выражение. В другом случае $3\sqrt{x^2-4x-5}=-2x \Leftrightarrow\begin{cases}9x^2-36x-45=4x^2,\\ x\leqslant0.\end{cases}\Leftrightarrow\begin{cases}5x^2-36x-45=0,\\ x\leqslant0.\end{cases}\Leftrightarrow\begin{cases}x=\cfrac{18\pm3\sqrt{61}}{5},\\ x\leqslant0.\end{cases}\Leftrightarrow x=\cfrac{18-3\sqrt{61}}{5}.$ Таким образом,\\ $x\in\left\{-2; \cfrac{18-3\sqrt{61}}{5}\right\}.$\\
