57. $\cfrac{x-4}{\sqrt{x}}-\cfrac{\sqrt{x}}{x-4}=\cfrac{8}{3}.$ Сделаем замену $t=\cfrac{x-4}{\sqrt{x}},$ тогда $t-\cfrac{1}{t}=\cfrac{8}{3},\ t^2-1=\cfrac{8}{3}t,\
 t^2-\cfrac{8}{3}t-1=0,\ t=-\cfrac{1}{3}$ или $t=3.$ В первом случае $\cfrac{x-4}{\sqrt{x}}=-\cfrac{1}{3},\ \sqrt{x}=12-3x,\ \begin{cases} x=144-72x+9x^2,\\ 12-3x\geqslant0.\end{cases}\Leftrightarrow\begin{cases} 9x^2-73x+144=0,\\ x\leqslant4.\end{cases}\Leftrightarrow x=\cfrac{73-\sqrt{145}}{18}.$ Во втором случае $
\cfrac{x-4}{\sqrt{x}}=3,\ \sqrt{x}=\cfrac{x-4}{3},$\\$ \begin{cases} x=\cfrac{x^2-8x+16}{9},\\ \cfrac{x-4}{3}\geqslant0.\end{cases}\Leftrightarrow
\begin{cases} x^2-17x+16=0,\\ x\geqslant4.\end{cases}\Leftrightarrow\begin{cases} (x-16)(x-1)=0,\\ x\geqslant4.\end{cases}\Leftrightarrow x=16.$\\