125. $(x^2-3x-4)\sqrt{x-2}=(x+1)(x^2-6x+8)\Leftrightarrow(x-4)(x+1)\sqrt{x-2}=(x+1)(x-2)(x-4)\Leftrightarrow
(x-4)(x+1)(\sqrt{x-2}-x+2)=0\Leftrightarrow
\begin{cases}\left[\begin{array}{l} x=4,\\ x=-1,\\ \sqrt{x-2}=x-2.\end{array}\right.\\ x\geqslant2.\end{cases}\Leftrightarrow
\begin{cases}\left[\begin{array}{l} x=4,\\ x-2=x^2-4x+4.\end{array}\right.\\ x\geqslant2.\end{cases}\Leftrightarrow
\begin{cases}\left[\begin{array}{l} x=4,\\ (x-2)(x-3)=0.\end{array}\right.\\ x\geqslant2.\end{cases}\Leftrightarrow x\in\{2;3;4\}$\\