127. $\left(x+\cfrac{1}{x}\right)^2-2x=3+\cfrac{2}{x}\Leftrightarrow \left(x+\cfrac{1}{x}\right)^2-2\left(x+\cfrac{1}{x}\right)-3=0\Leftrightarrow
\begin{cases} t=x+\cfrac{1}{x},\\ t^2-2t-3=0.\end{cases}\Leftrightarrow$\\$
\begin{cases} t=x+\cfrac{1}{x},\\ (t-3)(t+1)=0.\end{cases}\Rightarrow \left[\begin{array}{l} x+\cfrac{1}{x}=-1,\\ x+\cfrac{1}{x}=3.\end{array}\right.
\Rightarrow \left[\begin{array}{l} x^2+x+1=0,\\ x^2-3x+1=0.\end{array}\right.\Rightarrow x\in\left\{\cfrac{3\pm\sqrt{5}}{2}\right\}.$\\
