76. $\cfrac{4(x^2+1)}{x^2-10x+1}-\cfrac{5x}{x^2+1}+\cfrac{7}{2}=0\Leftrightarrow\cfrac{4}{1-10\cfrac{x}{x^2+1}}-5\cfrac{x}{x^2+1}+\cfrac{7}{2}=0.$ Сделаем замену $t=\cfrac{x}{x^2+1},$ тогда $\cfrac{4}{1-10t}-5t+\cfrac{7}{2}=0\Leftrightarrow 4-5t+50t^2+\cfrac{7}{2}-35t=0,\
50t^2-40t+\cfrac{15}{2}=0,\ 20t^2-16t+3=0,\ (2t-1)(10t-3)=0,\ t=\cfrac{1}{2}$ или $t=\cfrac{3}{10}.$ В первом случае $\cfrac{x}{x^2+1}=\cfrac{1}{2},\
2x=x^2+1,\ x^2-2x+1=0,\ (x-1)^2=0,\ x=1.$ Во втором случае $\cfrac{x}{x^2+1}=\cfrac{3}{10},\ 10x=3x^2+3,\ 3x^2-10x+3=0,\ (x-3)(3x-1)=0,\ x=\cfrac{1}{3}$ или $x=3.$\\
