147. $\left(\cfrac{4n+1}{2n^2+n-10}-\cfrac{4}{n^2-4}\right)\cdot\cfrac{4n^2+10n}{4n+9}+\cfrac{4}{n+2}=
\left(\cfrac{4n+1}{2(n^2-4)+n-2}-\cfrac{4}{(n-2)(n+2)}\right)\cdot\cfrac{2n(2n+5)}{4n+9}+\cfrac{4}{n+2}=
\left(\cfrac{4n+1}{2(n-2)(n+2)+n-2}-\cfrac{4}{(n-2)(n+2)}\right)\cdot\cfrac{2n(2n+5)}{4n+9}+\cfrac{4}{n+2}=$\\$
\left(\cfrac{4n+1}{(n-2)(2n+5)}-\cfrac{4}{(n-2)(n+2)}\right)\cdot\cfrac{2n(2n+5)}{4n+9}+\cfrac{4}{n+2}=
\cfrac{(4n+1)(n+2)-4(2n+5)}{(2n+5)(n-2)(n+2)}\cdot\cfrac{2n(2n+5)}{4n+9}+\cfrac{4}{n+2}=
\cfrac{4n^2+n-18}{(n-2)(n+2)}\cdot\cfrac{2n}{4n+9}+\cfrac{4}{n+2}=
\cfrac{4(n^2-4)+n-2}{(n-2)(n+2)}\cdot\cfrac{2n}{4n+9}+\cfrac{4}{n+2}=
\cfrac{(n-2)(4n+9)}{(n-2)(n+2)}\cdot\cfrac{2n}{4n+9}+\cfrac{4}{n+2}=\cfrac{2n}{n+2}+\cfrac{4}{n+2}=2.$\\
