86. $\cfrac{1}{x+2}+\cfrac{5}{x^2-x-6}+\cfrac{2x}{x-3}=\cfrac{1}{x+2}+\cfrac{5}{x(x-3)+2(x-3)}+\cfrac{2x}{x-3}=
\cfrac{1}{x+2}+\cfrac{5}{(x+2)(x-3)}+\cfrac{2x}{x-3}=$\\$=\cfrac{x-3+5+2x^2+4x}{(x+2)(x-3)}=\cfrac{2x^2+5x+2}{(x+2)(x-3)}=
\cfrac{2x^2+5x+2}{(x+2)(x-3)}=\cfrac{2x(x+2)+x+2}{(x+2)(x-3)}=\cfrac{(x+2)(2x+1)}{(x+2)(x-3)}=$\\$=\cfrac{2x+1}{x-3}.$\\
$\cfrac{2x+1}{x-3}:\cfrac{2x+1}{x}=\cfrac{2x+1}{x-3}\cdot\cfrac{x}{2x+1}=\cfrac{x}{x-3}.$\\
$\cfrac{x}{x-3}-\cfrac{x-9}{2(x-3)}=\cfrac{2x-x+9}{2(x-3)}=\cfrac{x+9}{2(x-3)}.$\\
