2. $\cfrac{6-3x}{2(1-x+x^2-x^3)}-\cfrac{2x^2+x-10}{2(x^3+x^2+x+1)}=
\cfrac{3(x-2)}{2(x^2(x-1)+(x-1))}-\cfrac{2(x^2-4)+x-2}{2(x^2(x+1)+x+1)}=$\\
$=\cfrac{3(x-2)}{2(x-1)(x^2+1)}-\cfrac{2(x-2)(x+2)+x-2}{2(x-1)(x^2+1)}=$\\
$=\cfrac{3(x-2)(x+1)}{2(x-1)(x^2+1)}-\cfrac{(x-2)(2(x+2)+1)(x-1)}{2(x+1)(x^2+1)}=\cfrac{(x-2)(3(x+1)-(2x+5)(x-1))}{2(x-1)(x+1)(x^2+1)}=$\\
$=\cfrac{(x-2)(8-2x^2)}{2(x-1)(x+1)(x^2+1)}=\cfrac{-2(x-2)^2(x+2)}{2(x-1)(x+1)(x^2+1)}=\cfrac{-(x-2)^2(x+2)}{(x-1)(x+1)(x^2+1)}.$\\
$\cfrac{5}{x^2+1}-\cfrac{3}{2(x-1)}+\cfrac{3}{2(x+1)}=\cfrac{5}{x^2+1}+\cfrac{3(x-1)}{2(x+1)(x-1)}-\cfrac{3(x+1)}{2(x+1)(x-1)}=
\cfrac{5}{x^2+1}+\cfrac{3x-3-3x-3}{2(x+1)(x-1)}=$\\$=\cfrac{5}{x^2+1}-\cfrac{6}{2(x+1)(x-1)}=\cfrac{5}{x^2+1}-\cfrac{3}{(x+1)(x-1)}=
\cfrac{5(x+1)(x-1)}{x^2+1}-\cfrac{3(x^2+1)}{(x+1)(x-1)(x^2+1)}=$\\$=\cfrac{5x^2-5-3x^2-3}{(x+1)(x-1)(x^2+1)}=
\cfrac{2(x-2)(x+2)}{(x+1)(x-1)(x^2+1)}.
$\\
$\cfrac{-(x-2)^2(x+2)}{(x-1)(x+1)(x^2+1)}:\cfrac{2(x-2)(x+2)}{(x+1)(x-1)(x^2+1)}=\cfrac{-(x-2)^2(x+2)}{(x-1)(x+1)(x^2+1)}\cdot\cfrac{(x+1)(x-1)(x^2+1)}{2(x-2)(x+2)}=\cfrac{2-x}{2}.$\\
