4. $\cfrac{\cfrac{1}{k}-\cfrac{1}{m-n}} {\cfrac{1}{k}+\cfrac{1}{m+n}}=\cfrac{\cfrac{m-n}{(m-n)k}-\cfrac{k}{(m-n)k}} {\cfrac{m+n}{(m+n)k}+\cfrac{k}{(m+n)k}}=
\cfrac{\cfrac{m-n-k}{(m-n)k}} {\cfrac{m+n+k}{(m+n)k}}=\cfrac{m-n-k}{(m-n)k}\cdot\cfrac{(m+n)k}{m+n+k}=\cfrac{(m-n-k)(m+n)}{(m+n+k)(m-n)}.$
$\cfrac{k^2+2nk}{m^2-n^2}-1=\cfrac{k^2+2nk-m^2+n^2}{m^2-n^2}=\cfrac{(n+k)^2-m^2}{(m-n)(m+n)}=\cfrac{(n+k-m)(n+k+m)}{(m-n)(m+n)}.$\\
$\left(1-\cfrac{k}{m+n+k}\right)^2=\left(\cfrac{m+n}{m+n+k}\right)^2=\cfrac{(m+n)^2}{(m+n+k)^2}.$\\
$\cfrac{(m-n-k)(m+n)}{(m+n+k)(m-n)}:\cfrac{(n+k-m)(n+k+m)}{(m-n)(m+n)}:\cfrac{(m+n)^2}{(m+n+k)^2}=$\\
$\cfrac{(m-n-k)(m+n)}{(m+n+k)(m-n)}\cdot\cfrac{(m-n)(m+n)}{(n+k-m)(n+k+m)}\cdot\cfrac{(m+n+k)^2}{(m+n)^2}=-1.$\\
