\section{Уравнения задачи}
$\begin{array}{ll}
1.\ \cfrac{3x-2}{x}+\cfrac{1}{2-x}=\cfrac{3x+4}{x^2-2x},&
2.\ \cfrac{1}{3-x}-\cfrac{2x+6}{x^2-3x}=\cfrac{2-5x}{x},\\
3.\ (x+5)^4+8(x+5)^2-9=0,&
4.\ (x-4)^4-3(x-4)^2-4=0,\\
5.\ \cfrac{6x}{x+1}=\cfrac{12x}{x^2-x+1}-\cfrac{12x^2-6x}{x^3+1},&
6.\ \cfrac{5x}{1-x}=\cfrac{10x}{x^2+x+1}+\cfrac{10x^2+5x}{1-x^3},\end{array}$ \\ $\begin{array}{ll}
7.\ \cfrac{3}{1+x+x^2}=3-x-x^2,&
8.\ \cfrac{2}{1+x+x^2}=2-x-x^2,\\
9.\ |x+1|+|x+2|=1,&
10.\ |x-1|+|x-2|=1,\\
11.\ (x+3)^2-|x+3|-30=0,&
12.\ (x-2)^2-3|x-2|-28=0,\end{array}$ \\ $\begin{array}{ll}
13.\ (x-1)^4-x^2+2x-73=0,&
14.\ (x+2)^4+2x^2+8x-16=0,\\
15.\ |x-3|+|x-5|=2,&
16.\ \cfrac{1}{x-5}-\cfrac{3}{x-3}=\cfrac{2}{x-4}-\cfrac{4}{x-2},\end{array}$ \\ $\begin{array}{ll}
17.\ \cfrac{3}{x-2}-\cfrac{4}{x-1}=\cfrac{1}{x-4}-\cfrac{2}{x-3},&
18.\ |3x+8|=x,\\
19.\ |2x+9|=x,&
20.\ \cfrac{1}{x+5}+\cfrac{1}{x+3}+\cfrac{1}{x-5}+\cfrac{1}{x-3}=0,\\
21.\ \cfrac{1}{x+4}+\cfrac{1}{x+2}+\cfrac{1}{x-4}+\cfrac{1}{x-2}=0,&
22.\ (x-1)^4-x^2+2x-13=0,\\
23.\ (x+1)^4-x^2-2x-13=0,&
24.\ |x^2-3x+5|=|4-2x-2x^2|,\\
25.\ \cfrac{2}{x-1}=\cfrac{x+5}{x^2+x-2},&
26.\ \cfrac{2}{x+1}=\cfrac{x-5}{x^2-x-2},\\
27.\ |x|-x+2=|2x-2|,&
28.\ |x|+x+2=|2x+2|,\\
29.\ \cfrac{x}{x-4}-\cfrac{1}{x+1}=\cfrac{2-x}{x+1}+\cfrac{3}{x-4},&
30.\ \cfrac{1}{x-1}+\cfrac{x}{x+4}=\cfrac{2+x}{1-x}-\cfrac{3}{x+4},\\
31.\ |5x-x^2-6|=x^2-5x-6,&
32.\ |5x-x^2-6|=5x-x^2-6,\end{array} \\ \begin{array}{ll}
33.\ \begin{cases}
x+2y=3,\\
x^2+y=2.\end{cases},&
34.\ \begin{cases}
x-2y=3,\\
x^2-y=2.\end{cases},\\
35.\ \cfrac{4x+8}{x^2-4}+2x+5=0,&
36.\ \cfrac{6x-18}{x^2-9}+2x-7=0,\\
37.\ (x^2-x+1)(2x^2-2x+1)=10,&
38.\ (x^2+x+1)(2x^2+2x+1)=10,\\
39.\ |x^2-10|=6,&
40.\ |x^2-17|=8,\\
41.\ \begin{cases}
x^2-16y^2+x+4y=0,\\
3x-4y=16.
\end{cases},&
42.\ \begin{cases}
x^2-9y^2+x-3y=0,\\
4x+3y=10.
\end{cases},\end{array}$\\ $\begin{array}{ll}
43.\ 2x^2+3x-17=2(2-\sqrt{7})^2+3(2-\sqrt{7})-17,&
44.\ x^2+2(1+\sqrt{8})x+8\sqrt{2}=0,\\
45.\ \cfrac{x}{x-2}+\cfrac{5}{x+2}=\cfrac{8}{x^2-4},&
46.\ \cfrac{x}{x+2}-\cfrac{5}{x-2}=\cfrac{8}{x^2-4},\\
47.\ (x+2)^3-x^3=2,&
48.\ (2-x)^3+x^3=2,\\
49.\ \cfrac{36}{4-x^2}+2=\cfrac{1-x}{x+2}-\cfrac{9}{x-2},&
50.\ \cfrac{3x}{x+3}-\cfrac{42}{x^2-9}=1+\cfrac{7}{3-x},\\
51.\ \cfrac{2x+1}{1+x}=\cfrac{2}{x^2-1},&
52.\ \cfrac{1-2x}{x-1}=\cfrac{-2}{x^2-1},\\
53.\ \sqrt{x-3}(3x^2-14x+8)=0,&
54.\ \sqrt{x-2}(3x^2-11x+6)=0,\\
55.\ 2|x+1|=|5-x|,&
56.\ 2|x+2|=|4-x|,\\
57.\ 2|2-x|=|x+7|,&
58.\ 3|3-x|=|x+1|,\\
59.\ \begin{cases}
xy+x^2=10,\\
xy+y^2=15.\end{cases},&
60.\ \begin{cases}
y^2-xy=4,\\
x^2-xy=-3.\end{cases},\\
61.\ (x^2-2x)^2-2x^2+4x=3,&
62.\ (x^2+2x)^2-2x^2-4x=3,\\
63.\ x^3-x^2+4x-4=0,&
64.\ x^3-x^2+5x-5=0,\end{array}\\ \begin{array}{ll}
65.\ \begin{cases}
0,4x+\cfrac{1}{3}y=1,8,\\
\cfrac{1}{5}x+0,27y=1,21.
\end{cases},&
66.\ \begin{cases}
0,4x-\cfrac{1}{3}y=1,8,\\
\cfrac{1}{5}x+0,27y=-0,41.
\end{cases},\\
67.\ |x-7|+|x-5|=x-4,&
68.\ |x-6|+|x-4|=x-3,\\
69.\ (x^2-2x-1)^2+3x^2-6x-13=0,&
70.\ \sqrt{(x-5)^2}=2x-6,\\
71.\ \sqrt{(x-7)^2}=4-3x,&
72.\ \cfrac{-2x^2+3-5x}{x+2}\cdot\sqrt{2-|x|}=0,\\
73.\ \cfrac{4+7x-2x^2}{x-3}\cdot\sqrt{3-|x|}=0,&
74.\ \sqrt{2x-x^2}+\sqrt{x^2-3x+2}+10x=20,\\
75.\ \sqrt{x-2}=100|x-3|+1,&
76.\ x^3+3x^2+3x+\cfrac{7}{8}=0,\\
77.\ 2x^2-3x-4=2(1+\sqrt{2})^2-3(1+\sqrt{2})-4,&
78.\ x^2-2x+1+\sqrt{7x-7}=0,\\
79.\ 2\left||x+4|-1\right|+6=30,&
80.\ (x-2)(x+1)(x+4)(x+7)=63,\end{array}\\ \begin{array}{ll}
81.\ \cfrac{2}{x^2+36+12x}-\cfrac{12}{36-x^2}=\cfrac{1}{x-6},&
82.\ 3x^2+2x+1=3(1-\sqrt{3})^2+2(1-\sqrt{3})+1,\\
83.\ 9x^3+3x^2+3x+1=0,&
84.\ x^3+x^2-4x-4=0,\end{array}\\ \begin{array}{lll}
85.\ |x-7|+|x^2-5|=x-4,&
86.\ 4x^4+3x^2-1=0,&
87.\ \begin{cases}
3x^2-y=7,\\
5y-3x^2=-23.
\end{cases},\\
88.\ x^3+x^2=2x,&
89.\ \begin{cases}
2x^2+xy=40,\\
3x-y=10.
\end{cases},
\end{array}$\\
$\begin{array}{ll}
90.\ \begin{cases}
x-y=3,\\
x^2y-xy^2=-6.
\end{cases},&
91.\ \begin{cases}
y-x=3,\\
x^2y-xy^2=6.
\end{cases},\\
92.\ x^2-6x+7+\cfrac{2}{x^2-6x+10}=0,&
93.\ x^2-3x-1+\cfrac{3}{x^2-3x+3}=0,\\
94.\ |x-1|=2x+1,&
95.\ |x+1|=1-2x,\\
96.\ x^4-3x^2-4=0,&
97.\ x^4+4x^2-5=0, \\
98.\ \cfrac{x+2}{2x-1}+\cfrac{x+1}{x+2}=\cfrac{9x-x^2+2}{2x^2+3x-2},&
99.\ |x^2-4x|=x^2+x-5,\\
100.\ |x^2+4x|=x^2-x-5,&
101.\ \begin{cases} x^2+3xy=1,\\ x-y=1.\end{cases}\\
102.\ \begin{cases} x^2+3xy=1,\\ x+y=1.\end{cases}&
103.\ \cfrac{2}{x-1}+\cfrac{1}{2}=\cfrac{-4}{x^2-4x+3},\\
104.\ \cfrac{1}{x-3}+\cfrac{1}{4}+\cfrac{2}{x^2-8x+15}=0.
\end{array}$\\
105. а) Решите уравнение $x^2-(\sqrt{2}+\sqrt{7})x+\sqrt{14}=0.$\\
б) Какой из корней этого уравнения ближе к числу 2?\\
106. а) Решите уравнение $x^2-(\sqrt{3}+\sqrt{5})x+\sqrt{15}=0.$\\
б) Какой из корней этого уравнения ближе к числу 2?\\
107. Упростить выражение $\left(\cfrac{\sqrt{x}+1}{\sqrt{x}-1}-\cfrac{\sqrt{x}-1}{\sqrt{x}+1}+4\sqrt{x}\right)\cdot\left(\sqrt{x}-\cfrac{1}{\sqrt{x}}\right)$ и определить при каких значениях $x$ это выражение равно выражению $x^2+3.$\\
$\begin{array}{ll}
108.\ (6x-3x^2-2)^5=(2-6x+3x^2)^{10},&
109.\ (x-2)^2-|x-2|-6=0,\\
110.\ x-\sqrt{x+1}-1=0,&
111.\ \cfrac{3}{(x-5)(x+2)}+\cfrac{5}{(x-4)(x+1)}=-2,\\
112.\ \cfrac{10}{(x-3)(x+6)}+\cfrac{9}{(x+4)(x-1)}=-1,&
113.\ |3x^2+18x-23|-|13-2x^2-12x|=-1,\\
114.\ |5x^2-20x-28|-|8x+9-2x^2|=-1,&
115.\ ||x^2-5|-1|=3,\\
116.\ |1-|x^2-6||=2,&
117.\ \left|\cfrac{4}{|x|-2}\right|=x-2,\\
118.\ \left|\cfrac{9}{|x|-3}\right|=x-3,&
119.\ x^2+x+\sqrt{x}-12=\sqrt{x},\\
120.\ 3x^2-2x-5=3(1-\sqrt{2})^2-2(1-\sqrt{2})-5,&
121.\ (x+1)\sqrt{x+3}-1=x,\\
122.\ \cfrac{6x}{x^3+4}+\cfrac{x}{x^3-3}=0,7x,&
123.\ \cfrac{6x}{x^3-4}+\cfrac{x}{x^3+3}=-0,7x,\\
124.\ \begin{cases} x^2+y^2-6x-8y=0,\\ x-4y=3.\end{cases},&
125.\ \begin{cases} x^2+y^2+8x-6y=0,\\ x-5y=-2.\end{cases}.
\end{array}$
\newpage
