21. $\cfrac{1}{x+4}+\cfrac{1}{x+2}+\cfrac{1}{x-4}+\cfrac{1}{x-2}=0\Leftrightarrow \cfrac{x+4+x-4}{(x+4)(x-4)}+\cfrac{x+2+x-2}{(x+2)(x-2)}=0\Leftrightarrow
\cfrac{2x}{x^2-16}+\cfrac{2x}{x^2-4}=0\Leftrightarrow 2x\cdot \cfrac{x^2-4+x^2-16}{(x^2-16)(x^2-4)}=0\Leftrightarrow 2x\cdot \cfrac{2(x+\sqrt{10})(x-\sqrt{10})}{(x^2-25)(x^2-9)}=0 \Leftrightarrow
    \left[
      \begin{gathered}
        x=0, \hfill
        \\
        x=-\sqrt{10}, \hfill
        \\
        x=\sqrt{10}. \hfill
      \end{gathered}
    \right. \hfill$\\
