16. $\cfrac{1}{x-5}-\cfrac{3}{x-3}=\cfrac{2}{x-4}-\cfrac{4}{x-2} \Leftrightarrow \cfrac{x-3-3x+15}{(x-5)(x-3)}=\cfrac{2x-4-4x+16}{(x-4)(x-2)}\Leftrightarrow$\\$
\cfrac{-2x+12}{(x-5)(x-3)}=\cfrac{-2x+12}{(x-4)(x-2)}\Leftrightarrow \begin{cases} \left[\begin{array}{l}-2x+12=0,\\
(x-5)(x-3)=(x-4)(x-2).\end{array}\right.\\ x\notin\{2;3;4;5\}\end{cases}\Leftrightarrow$\\$ \begin{cases} \left[\begin{array}{l}x=6,\\
x^2-3x-5x+15=x^2-2x-4x+8.\end{array}\right.\\ x\notin\{2;3;4;5\}\end{cases}\Leftrightarrow \begin{cases} \left[\begin{array}{l}x=6,\\
x=\cfrac{7}{2}.\end{array}\right.\\ x\notin\{2;3;4;5\}\end{cases}\Leftrightarrow\left[\begin{array}{l}x=6,\\
x=\cfrac{7}{2}.\end{array}\right.$\\