107. $\left(\cfrac{\sqrt{x}+1}{\sqrt{x}-1}-\cfrac{\sqrt{x}-1}{\sqrt{x}+1}+4\sqrt{x}\right)\cdot\left(\sqrt{x}-\cfrac{1}{\sqrt{x}}\right)=[a=\sqrt{x}]=
\left(\cfrac{a+1}{a-1}-\cfrac{a-1}{a+1}+4a\right)\cdot\left(a-\cfrac{1}{a}\right)=
\cfrac{a^2+2a+1-a^2+2a-1+4a^3-4a}{(a-1)(a+1)}\cdot\cfrac{a^2-1}{a}=
\cfrac{4a^3}{(a-1)(a+1)}\cdot\cfrac{(a-1)(a+1)}{a}=4a^2=4x.$ При этом $a\notin\{-1;0;1\},$ поэтому $x\notin\{0;1\}.$ Если $4x=x^2+3,$ то $x^2-4x+3=0,\ (x-1)(x-3)=0,\ x=1$ или $x=3,$ но $x$ не может быть равен 1, поэтому единственное решение --- $x=3.$\\
