111. $\cfrac{3}{(x-5)(x+2)}+\cfrac{5}{(x-4)(x+1)}=-2\Leftrightarrow
\cfrac{3}{x^2-3x-10}+\cfrac{5}{x^2-3x-4}=-2\Leftrightarrow\begin{cases} t=x^2-3x-4,\\ \cfrac{3}{t-6}+\cfrac{5}{t}=-2.\end{cases}$\\
$\Leftrightarrow\begin{cases} t=x^2-3x-4,\\ 3t+5t-30=-2t^2+12t.\end{cases}
\Leftrightarrow\begin{cases} t=x^2-3x-4,\\ t^2-2t-15=0.\end{cases}
\Leftrightarrow\begin{cases} t=x^2-3x-4,\\ (t-5)(t+3)=0.\end{cases}
\Leftrightarrow$\\$\left[\begin{array}{l}x^2-3x-4=5,\\ x^2-3x-4=-3.\end{array}\right.
\Leftrightarrow\left[\begin{array}{l}x^2-3x-9=0,\\ x^2-3x-1=0.\end{array}\right.
\Leftrightarrow x\in\left\{\cfrac{3\pm\sqrt{13}}{2}; \cfrac{3\pm3\sqrt{5}}{2}\right\}.$\\
