62. $(x^2+2x)^2-2x^2-4x=3\Leftrightarrow(x^2+2x)^2-2(x^2+2x)-3=0\Leftrightarrow\begin{cases}x^2+2x=t,\\ t^2-2t-3=0.\end{cases}
\Leftrightarrow\left[
      \begin{gathered}
      x^2+2x=-1,\hfill\\
      x^2+2x=3.\hfill
      \end{gathered}\right.\Leftrightarrow\left[
      \begin{gathered}
      x^2+2x+1=0,\hfill\\
      x^2+2x-3=0.\hfill
      \end{gathered}\right.\Leftrightarrow\left[
      \begin{gathered}
      x=-1,\hfill\\
      x=1,\hfill\\
      x=-3.\hfill
      \end{gathered}\right.$\\
