93. $x^2-3x-1+\cfrac{3}{x^2-3x+3}=0\Leftrightarrow \begin{cases}t-4+\cfrac{3}{t}=0,\\ t=x^2-3x+3\neq0.\end{cases}\Leftrightarrow
\begin{cases}t^2-4t+3=0,\\ t=x^2-3x+3\neq0.\end{cases}\Leftrightarrow$\\$\left[\begin{gathered}
     x^2-3x+3=1,\hfill\\
     x^2-3x+3=3.\hfill \end{gathered}\right.\Leftrightarrow\left[\begin{gathered}
     x^2-3x+2=0,\hfill\\
     x^2-3x=0.\hfill \end{gathered}\right.\Leftrightarrow\left[\begin{gathered}
     (x-2)(x-1)=0,\hfill\\
     x(x-3)=0.\hfill \end{gathered}\right.\Leftrightarrow x\in\{0;1;2;3\}.$\\
