112. $\cfrac{10}{(x-3)(x+6)}+\cfrac{9}{(x+4)(x-1)}=-1\Leftrightarrow
\cfrac{10}{x^2+3x-18}+\cfrac{9}{x^2+3x-4}=-1\Leftrightarrow\begin{cases} t=x^2+3x-4,\\ \cfrac{10}{t-14}+\cfrac{9}{t}=-1.\end{cases}$\\
$\Leftrightarrow\begin{cases} t=x^2+3x-4,\\ 10t+9t-126=-t^2+14t.\end{cases}
\Leftrightarrow\begin{cases} t=x^2+3x-4,\\ t^2+5t-126=0.\end{cases}
\Leftrightarrow\begin{cases} t=x^2+3x-4,\\ (t+14)(t-9)=0.\end{cases}
\Leftrightarrow$\\$\left[\begin{array}{l}x^2+3x-4=-14,\\ x^2+3x-4=9.\end{array}\right.
\Leftrightarrow\left[\begin{array}{l}x^2+3x+10=0,\\ x^2+3x-13=0.\end{array}\right.
\Leftrightarrow x\in\left\{\cfrac{-3\pm\sqrt{61}}{2}\right\}.$\\