20. $\cfrac{1}{x+5}+\cfrac{1}{x+3}+\cfrac{1}{x-5}+\cfrac{1}{x-3}=0\Leftrightarrow \cfrac{x+5+x-5}{(x+5)(x-5)}+\cfrac{x+3+x-3}{(x+3)(x-3)}=0\Leftrightarrow
\cfrac{2x}{x^2-25}+\cfrac{2x}{x^2-9}=0\Leftrightarrow 2x\cdot \cfrac{x^2-9+x^2-25}{(x^2-25)(x^2-9)}=0\Leftrightarrow 2x\cdot \cfrac{2(x+\sqrt{17})(x-\sqrt{17})}{(x^2-25)(x^2-9)}=0 \Leftrightarrow
    \left[
      \begin{gathered}
        x=0, \hfill
        \\
        x=-\sqrt{17}, \hfill
        \\
        x=\sqrt{17}. \hfill
      \end{gathered}
    \right. \hfill$\\
