80. $(x-2)(x+1)(x+4)(x+7)=63\Leftrightarrow (x^2+7x-2x-14)(x^2+4x+x+4)=63\Leftrightarrow (x^2+5x-14)(x^2+5x+4)=63\Leftrightarrow
\begin{cases}t=x^2+5x,\\ (t-14)(t+4)=63.\end{cases}\Leftrightarrow
\begin{cases}t=x^2+5x,\\ t^2+4t-14t-56=63.\end{cases}\Leftrightarrow
\begin{cases}t=x^2+5x,\\ t^2-10t-119=0.\end{cases}\Leftrightarrow
\begin{cases}t=x^2+5x,\\ (t-17)(t+7)=0.\end{cases}\Leftrightarrow\left[
      \begin{gathered} x^2+5x=17,\hfill\\
      x^2+5x=-7.\hfill \end{gathered}\right.\Leftrightarrow\left[
      \begin{gathered} x^2+5x-17=0,\hfill\\
      x^2+5x+7=0.\hfill \end{gathered}\right.\Leftrightarrow x=\cfrac{-5\pm\sqrt{93}}{2}.$\\