60. $\begin{cases}
y^2-xy=4,\\
x^2-xy=-3.\end{cases}\Leftrightarrow\begin{cases}
x^2-xy=-3,\\
x^2-2xy+y^2=1.\end{cases}\Leftrightarrow\begin{cases}
x^2-xy=-3,\\
(x-y)^2=1.\end{cases}\Leftrightarrow\left[
      \begin{gathered} \begin{cases}x^2-xy=-3,\\ x-y=1.\end{cases}\hfill\\
      \begin{cases}x^2-xy=-3,\\ x-y=-1.\end{cases}\hfill \end{gathered}\right.
\Leftrightarrow$\\$\left[
      \begin{gathered} \begin{cases}x^2-x^2+x=-3,\\ y=x-1.\end{cases}\hfill\\
      \begin{cases}x^2-x^2-x=-3,\\ y=x+1.\end{cases}\hfill \end{gathered}\right.
\Leftrightarrow\left[
      \begin{gathered} \begin{cases}x=-3,\\ y=-4.\end{cases}\hfill\\
      \begin{cases}x=3,\\ y=4.\end{cases}\hfill \end{gathered}\right.$\\