92. $y=\cfrac{2x^3+x^2-2x-1}{1-x^2}=\cfrac{x^2(2x+1)-(2x+1)}{1-x^2}=\cfrac{(2x+1)(x^2-1)}{1-x^2}=-2x-1,\ x\neq\pm1.$
$$\begin{tikzpicture}[scale=0.2]
\tikzset {line01/.style={line width =0.5pt}}
\tikzset{line02/.style={line width =1pt}}
\tikzset{line03/.style={dashed,line width =0.5pt}}
%\filldraw [black] (0,0) circle (1pt);
\draw [->] (-10,0) -- (10,0);
\draw [->] (0,-10) -- (0,10);
\draw[line01] (-5,9) -- (4,-9);
\draw (10.2,0.7) node {\scriptsize $x$};
\draw (-1.2,-1.3) node {\scriptsize $-1$};
\draw (1.2,0.7) node {\scriptsize $1$};
\draw (0.4,1) node {\scriptsize $1$};
\draw (-1.1,-3) node {\scriptsize $-3$};
%\draw (0.7,6) node {\scriptsize $6$};
%\draw (-5.5,-2) node {\scriptsize $-6$};
\draw[line03] (-1,0) -- (-1,1);
\draw[line03] (-0.9,1) -- (0,1);
\draw[line03] (1,0) -- (1,-3);
\draw[line03] (1,-3) -- (0,-3);

\draw (0.7,10.2) node {\scriptsize $y$};
\draw (1,-3) circle (10pt);
\draw (-1,1) circle (10pt);
\end{tikzpicture}$$
