93. $y=\cfrac{x^3-x^2-x+1}{1-x^2}=\cfrac{x^2(x-1)-(x-1)}{1-x^2}=\cfrac{(x-1)(x^2-1)}{1-x^2}=1-x,\ x\neq\pm1.$
$$\begin{tikzpicture}[scale=0.2]
\tikzset {line01/.style={line width =0.5pt}}
\tikzset{line02/.style={line width =1pt}}
\tikzset{line03/.style={dashed,line width =0.5pt}}
%\filldraw [black] (0,0) circle (1pt);
\draw [->] (-10,0) -- (10,0);
\draw [->] (0,-10) -- (0,10);
\draw[line01] (-7,8) -- (4,-3);
\draw (10.2,0.7) node {\scriptsize $x$};
\draw (-1.2,-1.3) node {\scriptsize $-1$};
\draw (1.2,0.9) node {\scriptsize $1$};
\draw (0.4,2) node {\scriptsize $2$};

%\draw (0.7,6) node {\scriptsize $6$};
%\draw (-5.5,-2) node {\scriptsize $-6$};
\draw[line03] (-1,0) -- (-1,2);
\draw[line03] (-0.9,2) -- (0,2);


\draw (0.7,10.2) node {\scriptsize $y$};
\draw (1,0) circle (10pt);
\draw (-1,2) circle (10pt);
\end{tikzpicture}$$\\
