82. $\cfrac{((x^2-4)^2+y^2-2y+1)(y^2-3xy+2x^2)}{xy-2y+3x-6}=0\Leftrightarrow
\begin{cases}

((x^2-4)^2+y^2-2y+1)(y^2-3xy+2x^2)=0,\\
xy-2y+3x-6\neq0.
\end{cases}$\\$\Leftrightarrow
\begin{cases}
\left[\begin{array}{l}
(x^2-4)^2+(y-1)^2=0,\\
y(y-x)+2x(x-y)=0,
\end{array}\right.\\
y(x-2)+3(x-2)\neq0.
\end{cases}\Leftrightarrow
\begin{cases}
\left[\begin{array}{l}
\begin{cases}
x^2-4=0,\\
y-1=0.
\end{cases}\\
(y-x)(y-2x)=0,
\end{array}\right.\\
(x-2)(y+3)\neq0.
\end{cases}\Leftrightarrow
\begin{cases}
\left[\begin{array}{l}
\begin{cases}
x=2,\\
y=1.
\end{cases}\\
\begin{cases}
x=-2,\\
y=1.
\end{cases}\\
y=x,\\
y=2x,
\end{array}\right.\\
x\neq2,\\
y\neq-3.
\end{cases}$
{{PIC:gr7-82.png}}\newpage\noindent
