23. $\left(\cfrac{\sqrt{x}-\sqrt{y}}{x\sqrt{y}+\sqrt{x}y}+\cfrac{\sqrt{x}+\sqrt{y}}{x\sqrt{y}-\sqrt{x}y}\right)
\cdot\cfrac{\sqrt{x^3}\sqrt{y}}{x+y}=[a=\sqrt{x},\ b=\sqrt{y}]=
\left(\cfrac{a-b}{a^2b+ab^2}+\cfrac{a+b}{a^2b-ab^2}\right)\cdot\cfrac{a^3b}{a^2+b^2}=
\left(\cfrac{a-b}{ab(a+b)}+\cfrac{a+b}{ab(a-b)}\right)\cdot\cfrac{a^3b}{a^2+b^2}=
\cfrac{a^2-2ab+b^2+a^2+2ab+b^2}{ab(a-b)(a+b)}\cdot\cfrac{a^3b}{a^2+b^2}=
\cfrac{2(a^2+b^2)}{ab(a-b)(a+b)}\cdot\cfrac{a^3b}{a^2+b^2}=\cfrac{2a^2}{a^2-b^2}=\cfrac{2x}{x-y}.$\\
