46. $\left(\cfrac{a^{\frac{3}{2}}+b^{\frac{3}{2}}}{a^{\frac{1}{2}}+b^{\frac{1}{2}}}-(a+b)\right)\cdot\cfrac{b^{\frac{1}{2}}-a^{\frac{1}{2}}}{a^{\frac{1}{2}}b^{\frac{3}{2}}-b^{\frac{1}{2}}a^{\frac{3}{2}}}=
[x=a^{\frac{1}{2}}, y=b^{\frac{1}{2}}]=
\left(\cfrac{x^3+y^3}{x+y}-(x^2+y^2)\right)\cdot\cfrac{y-x}{xy^3-yx^3}=$\\$\left(\cfrac{(x+y)(x^2-xy+y^2)}{x+y}-x^2-y^2\right)\cdot\cfrac{y-x}{xy(y-x)(y+x)}=
\left(x^2-xy+y^2-x^2-y^2\right)\cdot\cfrac{1}{xy(y+x)}=$\\$-xy\cdot\cfrac{1}{xy(y+x)}=-\cfrac{1}{x+y}=-\cfrac{1}{a^{\frac{1}{2}}+b^{\frac{1}{2}}}=\cfrac{\sqrt{b}-\sqrt{a}}{a-b}.$\\
