19. $\left(\cfrac{\sqrt{a}-2}{a+2\sqrt{a}}+\cfrac{\sqrt{a}+2}{a-2\sqrt{a}}\right)\cdot
\cfrac{a^\frac{3}{2}}{a+4}-\cfrac{8}{a-4}=[x=\sqrt{a}]=
\left(\cfrac{x-2}{x^2+2x}+\cfrac{x+2}{x^2-2x}\right)\cdot\cfrac{x^3}{x^2+4}-\cfrac{8}{x^2-4}=
\left(\cfrac{x-2}{x(x+2)}+\cfrac{x+2}{x(x-2)}\right)\cdot\cfrac{x^3}{x^2+4}-\cfrac{8}{x^2-4}=
\cfrac{x^2-4x+4+x^2+4x+4}{x(x+2)(x-2)}\cdot\cfrac{x^3}{x^2+4}-\cfrac{8}{x^2-4}=
\cfrac{2(x^2+4)}{x(x+2)(x-2)}\cdot\cfrac{x^3}{x^2+4}-\cfrac{8}{x^2-4}=
\cfrac{2x^2}{(x+2)(x-2)}-\cfrac{8}{(x+2)(x-2)}=\cfrac{2x^2-8}{(x+2)(x-2)}=\cfrac{2(x-2)(x+2)}{(x+2)(x-2)}=2.$\\