2. $a^{\frac{4}{3}}\cdot\left(\cfrac{3}{\sqrt[3]{a^2}-\sqrt[3]{a}+1}-
\cfrac{3}{a+1}+\cfrac{\sqrt[3]{a}-1}{\sqrt[3]{a^2}-1}\right)^{-1}
\left(\cfrac{a^{-\frac{1}{3}}+1}{a^\frac{1}{3}}\right)^2=[x=\sqrt[3]{a}]=$\\$
x^4\cdot\left(\cfrac{3}{x^2-x+1}-\cfrac{3}{x^3+1}+\cfrac{x-1}{x^2-1}\right)^{-1}\left(\cfrac{\cfrac{1}{x}+1}{x}\right)^2=$\\$
x^4\cdot\left(\cfrac{3}{x^2-x+1}-\cfrac{3}{(x+1)(x^2-x+1)}+\cfrac{1}{x+1}\right)^{-1}\left(\cfrac{x+1}{x^2}\right)^2=$\\$
x^4\cdot\left(\cfrac{3x+3-3+x^2-x+1}{(x+1)(x^2-x+1)}\right)^{-1}\cfrac{(x+1)^2}{x^4}=
\left(\cfrac{(x+1)^2}{(x+1)(x^2-x+1)}\right)^{-1}(x+1)^2=\cfrac{x^3+1}{(x+1)^2}(x+1)^2=x^3+1=a+1.$\\
